sweep coalescing proof completed,  little clean up required

Proofs/Spec.GC_infix_closure_ver3.fst
@@ -11,8 +11,6 @@ open FStar.FunctionalExtensionality
 //Machine integer
 module Usize = FStar.UInt64
 
-let heap_size = admit ()
-
 let max_wosize_lemma () =
    assert (Usize.v (Usize.shift_left 1UL 54ul) == pow2 54 % pow2 64);
    Math.Lemmas.pow2_lt_compat 64 54;
@@ -30,7 +28,7 @@ let max_tag_size_lemma () =
 
 let is_size_fits_after_subtraction x y = UInt.fits (Usize.v x - Usize.v y) Usize.n
 
-let getWosize h =
+let getWosize h = 
  let _ = max_wosize_lemma () in
  let _ = assert (Usize.v max_wosize = pow2 54 - 1) in
  let wz = Usize.shift_right h 10ul in
@@ -38,8 +36,8 @@ let getWosize h =
  assert (Usize.v wz <= Usize.v max_wosize);
  assert (Usize.v wz >= 0);
  wz
-
-let getColor h =
+ 
+let getColor h = 
  let _ = max_color_size_lemma () in
  let _ = assert (Usize.v max_color = pow2 2 - 1) in
  let c' = Usize.shift_right h 8ul in
@@ -58,7 +56,7 @@ let getColor h =
  assert (Usize.v max_color <= pow2 64 - 1);
  c
 
-let getTag h =
+let getTag h = 
  let _ = max_tag_size_lemma () in
  assert (Usize.v max_tag = pow2 8 - 1);
  let t = Usize.logand h 255UL in
@@ -66,44 +64,44 @@ let getTag h =
  assert (Usize.v max_tag <= pow2 8 - 1);
  assert (Usize.v t <= 255);
  assert (Usize.v t <= Usize.v max_tag);
- t
+ t     
 
 let color_of_object1 v_id g =
-
-  let hd_val = read_word g v_id in
+  
+  let hd_val = read_word g v_id in 
   let c = getColor (hd_val) in
   c
 
 let wosize_of_object1 v_id g =
-
-  let hd_val = read_word g v_id in
+  
+  let hd_val = read_word g v_id in 
   let w = getWosize (hd_val) in
   w
 
 let tag_of_object1 v_id g =
-
-  let hd_val = read_word g v_id in
+  
+  let hd_val = read_word g v_id in 
   let t = getTag (hd_val) in
   t
 
-let isBlueObject1 v_id g =
+let isBlueObject1 v_id g = 
  if color_of_object1 v_id g = blue then true
- else
+ else 
   false
 
-let isWhiteObject1 v_id g =
+let isWhiteObject1 v_id g = 
  if color_of_object1 v_id g = white then true
- else
+ else 
   false
 
-let isGrayObject1 v_id g =
+let isGrayObject1 v_id g = 
   if color_of_object1 v_id g = gray then true
- else
+ else 
   false
 
-let isBlackObject1 v_id g =
+let isBlackObject1 v_id g = 
    if color_of_object1 v_id g = black then true
- else
+ else 
   false
 
 open FStar.UInt
@@ -113,7 +111,7 @@ open FStar.UInt
 
 #push-options "--split_queries always"
 
-let makeHeader wz c tg =
+let makeHeader wz c tg = 
  let l1 = Usize.shift_left wz 10ul in
  let l2 = Usize.shift_left c 8ul in
  let l3 = Usize.shift_left tg 0ul in
@@ -126,7 +124,7 @@ let makeHeader wz c tg =
  assert (Usize.v wz < pow2 54);
  assert (Usize.v c < pow2 2);
  assert (Usize.v tg < pow2 8);
-
+ 
  //Prove that wz shifted to left 10 positions is less than pow2 32. So when we take mod of pow2 32, the shift will not overflow
 // Math.Lemmas.lemma_mult_lt_right (pow2 10) (Usize.v wz) (pow2 22);
  assert (pow2 10 > 0);
@@ -140,7 +138,7 @@ let makeHeader wz c tg =
 
  assert (Usize.v l2 == Usize.v c * pow2 8);
  assert (Usize.v l3 == Usize.v tg * pow2 0);
-
+ 
  let s = Usize.add (Usize.add l1 l2) l3 in
  assert (Usize.v s < pow2 64);
  assert (Usize.v l1 < pow2 64);
@@ -159,7 +157,7 @@ let makeHeader wz c tg =
  assert (Usize.v l1' == Usize.v wz);
 
  assert (Usize.v l2' == Usize.v c * (pow2 8/pow2 10));
-
+ 
  assert (pow2 8 < pow2 10);
  assert (Usize.v l3' == Usize.v tg * (pow2 0/pow2 10));
  let s1' =  Usize.shift_right s 10ul in
@@ -180,7 +178,7 @@ let makeHeader wz c tg =
  assert (Usize.v l1'' == (Usize.v wz * pow2 10)/pow2 8);
  Math.Lemmas.pow2_minus 10 8;
  assert (Usize.v l1'' == Usize.v wz * pow2 2);
-
+ 
  assert (Usize.v l2'' == (Usize.v c * pow2 8 )/pow2 8);
  Math.Lemmas.cancel_mul_div (Usize.v c) (pow2 8);
  assert (Usize.v l2'' == Usize.v c);
@@ -196,9 +194,9 @@ let makeHeader wz c tg =
  assert (Usize.v s2 == ((Usize.v wz * pow2 10)/pow2 8) + ((Usize.v c * pow2 8)/pow2 8));
  assert (Usize.v s2 == ((Usize.v wz * pow2 10)/pow2 8) + Usize.v c);
  assert (Usize.v s2 == (Usize.v wz * pow2 2) + Usize.v c);
-
+ 
  //assert (Usize.v s2 == Usize.v l1'' + Usize.v l2'' + Usize.v l3'');
-
+ 
  let s2' = Usize.logand s2 3UL in
 
  assert (pow2 2 - 1 == 3);
@@ -207,11 +205,11 @@ let makeHeader wz c tg =
  assert (Usize.v c < pow2 2);
  assert ((Usize.v wz * pow2 2) % pow2 2 == 0);
  assert (Usize.v s2' == Usize.v c);
-
+ 
  let s3' = Usize.logand s 255UL in
  logand_mask #64 (Usize.v s) 8;
-
- assert (s2' == c);
+ 
+ assert (s2' == c); 
  assert (s3' == tg);
  assert (getColor s == s2');
  assert (getTag s == s3');
@@ -227,9 +225,9 @@ let makeHeader wz c tg =
 #push-options "--z3rlimit 100 --fuel 2 --ifuel 1"
 
 let isPointer v_id g =
-  if Usize.logand (read_word g v_id) 1UL = 0UL then true else false
+  if Usize.logand (read_word g v_id) 1UL = 0UL then true else false 
 
-let is_fields_within_limit1 h_index wz =
+let is_fields_within_limit1 h_index wz = 
  //let s = Usize.add h_index (Usize.mul wz mword) in
  let s1 = Usize.add wz 1UL in // s1 = (wz + 1)
  let s2 = Usize.mul s1 mword in //s2 = (s1 * mword)
@@ -242,7 +240,7 @@ let is_fields_within_limit1 h_index wz =
 
 #push-options "--split_queries always"
 
-let rec is_fields_contents_within_limit2 h_index wz g =
+let rec is_fields_contents_within_limit2 h_index wz g = 
     if (Usize.v wz = 0) then true
     else
       (
@@ -264,7 +262,7 @@ let rec is_fields_contents_within_limit2 h_index wz g =
        )
 
 
-
+ 
 
 
 let color_lemma (h_index)
@@ -279,12 +277,12 @@ let color_lemma (h_index)
 
 #restart-solver
 
-#restart-solver
+#restart-solver 
 
 let rec objects2 h_index g =
 let wz =  getWosize (read_word g h_index) in
 let h_index_new =  Usize.add h_index (Usize.mul (Usize.add wz 1UL) mword) in
-if Usize.v wz = 0 then
+if Usize.v wz = 0 then 
 (
   let f' = Seq.empty  in// There are no zero length objects.
   assert (Seq.length f' > 0 /\ (Usize.v h_index_new < heap_size) ==> Seq.mem h_index_new f');
@@ -302,7 +300,7 @@ else
     (
        assert (Usize.v h_index_new == heap_size);
        let f = Seq.create 1 h_index in
-
+       
        G.is_vertex_set_lemma2 f;
        assert (Seq.length f > 0 /\ (Usize.v h_index_new < heap_size) ==> Seq.mem h_index_new f);
        assert (forall x. Seq.mem x f ==> is_hp_addr x);
@@ -310,10 +308,10 @@ else
     )
     else
     (
-      assert (Usize.v h_index_new < heap_size);
+      assert (Usize.v h_index_new < heap_size); 
       let f_index_new =  Usize.add h_index_new mword in
-      let f' =  objects2 h_index_new g in
-      if length f' = 0 ||  (Usize.v f_index_new = heap_size) then
+      let f' =  objects2 h_index_new g in 
+      if length f' = 0 ||  (Usize.v f_index_new = heap_size) then 
       (
         assert (Seq.length f' > 0 /\ (Usize.v h_index_new < heap_size) ==> Seq.mem h_index_new f');
         assert (forall x. Seq.mem x f' ==> is_hp_addr x);
@@ -342,22 +340,753 @@ else
   )
 )
 
-let wosize_plus_times_mword_multiple_of_mword (wz:wosize)
-                     :Lemma
+#restart-solver
+
+#restart-solver
+
+let rec objects2_empty_lemma (h_index: hp_addr)
+                             (g:heap) 
+                : Lemma
+                  (requires True)
+                  (ensures (Seq.length (objects2 h_index g) == 0 ==>
+                              (exists (p:hp_addr). Usize.v p >= Usize.v h_index /\ 
+                                ((Usize.v (getWosize (read_word g p)) == 0) \/
+                                  Usize.v (Usize.add p (Usize.mul (Usize.add (getWosize (read_word g p)) 1UL) mword)) > heap_size))))
+                   (decreases (heap_size - Usize.v h_index)) =
+let wz =  getWosize (read_word g h_index) in
+let h_index_new =  Usize.add h_index (Usize.mul (Usize.add wz 1UL) mword) in
+if Usize.v wz = 0 then 
+(
+  assert (Seq.length (objects2 h_index g) == 0 ==>
+                 (exists (p:hp_addr). Usize.v p >= Usize.v h_index /\ 
+                     ((Usize.v (getWosize (read_word g p)) == 0) \/
+                      Usize.v (Usize.add p (Usize.mul (Usize.add (getWosize (read_word g p)) 1UL) mword)) > heap_size)));
+  ()
+)
+else
+(
+  if Usize.v h_index_new <= heap_size then
+  (
+    if Usize.v h_index_new = heap_size then
+    (
+      assert (Seq.length (objects2 h_index g) > 0);
+      assert (Seq.length (objects2 h_index g) == 0 ==>
+                 (exists (p:hp_addr). Usize.v p >= Usize.v h_index /\ 
+                     ((Usize.v (getWosize (read_word g p)) == 0) \/
+                      Usize.v (Usize.add p (Usize.mul (Usize.add (getWosize (read_word g p)) 1UL) mword)) > heap_size)));
+      ()
+    )
+    else
+    (
+      let f' =  objects2 h_index_new g in 
+      objects2_empty_lemma h_index_new g;
+      assert (Seq.length (objects2 h_index_new g) == 0 ==>
+                 (exists (p:hp_addr). Usize.v p >= Usize.v h_index_new /\ 
+                     ((Usize.v (getWosize (read_word g p)) == 0) \/
+                      Usize.v (Usize.add p (Usize.mul (Usize.add (getWosize (read_word g p)) 1UL) mword)) > heap_size)));
+      
+      if length f' = 0 then
+      (
+        assert (Seq.length (objects2 h_index g) == 0 ==>
+                 (exists (p:hp_addr). Usize.v p >= Usize.v h_index /\ 
+                     ((Usize.v (getWosize (read_word g p)) == 0) \/
+                      Usize.v (Usize.add p (Usize.mul (Usize.add (getWosize (read_word g p)) 1UL) mword)) > heap_size)));
+        ()
+      )
+      else
+      (
+        assert (Seq.length (objects2 h_index g) == 0 ==>
+                 (exists (p:hp_addr). Usize.v p >= Usize.v h_index /\ 
+                     ((Usize.v (getWosize (read_word g p)) == 0) \/
+                      Usize.v (Usize.add p (Usize.mul (Usize.add (getWosize (read_word g p)) 1UL) mword)) > heap_size)));
+        ()
+      )
+    )
+  )
+  else
+  (
+    assert (Seq.length (objects2 h_index g) == 0 ==>
+                 (exists (p:hp_addr). Usize.v p >= Usize.v h_index /\ 
+                     ((Usize.v (getWosize (read_word g p)) == 0) \/
+                      Usize.v (Usize.add p (Usize.mul (Usize.add (getWosize (read_word g p)) 1UL) mword)) > heap_size)));
+    ()
+  )
+)
+
+let heap_remains_same_except_index_v_id1  (v_id:hp_addr)
+                                         (g:heap)
+                                         (g':heap{Seq.length g == Seq.length g'}) =
+  forall (x:Usize.t {Usize.v x < heap_size /\ (Usize.v x % Usize.v mword == 0)}). x <> v_id ==>
+           read_word g x == read_word g' x 
+
+#restart-solver
+
+#restart-solver
+
+#restart-solver
+
+let wosize_times_mword_multiple_of_mword1 (wz:wosize)
+                     :Lemma 
                       (ensures (Usize.v (Usize.mul (Usize.add wz 1UL) mword) % Usize.v mword == 0)) = ()
 
+
+let rec objects2_non_empty_lemma (h_index: hp_addr)
+                                 (g:heap) 
+                                 (g1:heap)
+                                 (fp:hp_addr{Usize.v fp >= Usize.v mword})
+                                 (f_index:hp_addr{Usize.v f_index >= Usize.v mword
+                                                  })
+                : Lemma
+                  (requires ( (* length of obj set of g > 0*)
+                              Seq.length (objects2 h_index g) > 0 /\
+
+                              (* heap differs only in header of fp between g and g1*)
+                              heap_remains_same_except_index_v_id1 (hd_address fp) g g1 /\
+                             
+                              
+                             ((* header of f_index*)
+                              let hd_index = hd_address f_index in
+
+                              (* wosize of f_index in g*)
+                              let wz = getWosize (read_word g hd_index) in
+                              
+                              (* header of fp*)
+                              let hd_fp = hd_address fp in
+
+                              (*wosize of fp in g *)
+                              let cur_wosize = getWosize (read_word g hd_fp) in
+
+                              (* wosize of f_index and wosize of fp together*)
+                              let combined_wz = Usize.add cur_wosize wz in
+
+                              (* the combined wosize + 1 will be the coalesced wosize, so that now f_index header is also a field 
+                                 of fp after coalescing*)
+                              let combined_wz_plus_one = Usize.add combined_wz 1UL in
+
+                               (*The new wosize added to header of fp resulted into the new heap g1*)
+                               (* Therefore, new wosize of hd_fp in g1 is combined wosize + 1 *)
+                              ((getWosize (read_word g1 hd_fp) == combined_wz_plus_one) /\
+                                 
+                                 (* the header of f_index is the next header of fp in g*)
+                                 hd_index == Usize.add hd_fp (Usize.mul (Usize.add cur_wosize 1UL) mword) /\
+
+                                 (* the combined wosize + 1 should be less than heap size in the original heap g *)
+                                 (* Otherwise, that means, either objects f_index has 
+                                    zero length fields (in that case, combined wosize + 1 = heapsize) or
+                                    the length of the fields exceed heap size (in that case, combined wosize + 1 > heapsize)
+                                    Both are contradicting cases with the fact that length of obj set of g > 0 and when
+                                    f_index and fp are valid objects of the object set of g. Don't put the facts that they are
+                                    valid objects of g here, because it affects inductive proof, as the induction is on an address and
+                                    it can be the case that during address change when induction happens, the membership property
+                                    can get violated. Therefore, instead of pasing the membership property explicitly,
+                                    pass the property that is derived from membership property, that is free of the induction variable.
+                                    And that property is,the combined wosize + 1 should be less than heap size in the original heap g *)
+                                Usize.v combined_wz_plus_one < heap_size /\
+
+                                (* The next header of f_index can be <= heap_size*)
+                                Usize.v (Usize.add hd_index (Usize.mul (Usize.add wz 1UL) mword)) <= heap_size)))
+                               )
+                  (ensures  (Seq.length (objects2 h_index g1) > 0))
+                  (decreases (heap_size - Usize.v h_index)) =
+  let wz =  getWosize (read_word g h_index) in
+  let h_index_new =  Usize.add h_index (Usize.mul (Usize.add wz 1UL) mword) in
+  
+  wosize_times_mword_multiple_of_mword1 wz;
+  sum_of_multiple_of_mword_is_multiple_of_mword h_index (Usize.mul (Usize.add wz 1UL) mword);
+
+  let wz1 =  getWosize (read_word g1 h_index) in
+  let hd_fp = hd_address fp in
+  if h_index <> hd_fp then
+  (
+    assert (heap_remains_same_except_index_v_id1 (hd_address fp) g g1);
+    assert (wz == wz1);
+    assert (Usize.v wz <> 0);
+    if Usize.v h_index_new <= heap_size then
+    (
+      if Usize.v h_index_new = heap_size then
+      (
+        ()
+      )
+      else
+      (
+        assert (is_hp_addr h_index_new);
+        let f' =  objects2 h_index_new g1 in 
+        objects2_non_empty_lemma h_index_new g g1 fp f_index;
+        assert (Seq.length (objects2 h_index_new g1) > 0);
+        ()
+      )
+    )
+    else
+    (
+      ()
+    )
+  )
+  else
+  (
+    assert (h_index == hd_fp);
+    let hd_index = hd_address f_index in
+    let wz_f_index = getWosize (read_word g hd_index) in
+    let hd_fp = hd_address fp in
+    let cur_wosize = getWosize (read_word g hd_fp) in
+    let combined_wz = Usize.add cur_wosize wz_f_index in
+    let combined_wz_plus_one = Usize.add combined_wz 1UL in
+    let new_fp_wosize = getWosize (read_word g1 hd_fp) in
+    assert (new_fp_wosize == combined_wz_plus_one);
+    assert (Usize.v combined_wz_plus_one > 0);
+    let h_index_new1 = Usize.add h_index (Usize.mul (Usize.add combined_wz_plus_one 1UL) mword) in
+    assert (Usize.v combined_wz_plus_one < heap_size);
+    let next_hd_index = Usize.add hd_index (Usize.mul (Usize.add wz_f_index 1UL) mword) in
+    (* h_index + (combined_wz_plus_one + 1) * mword
+       h_index + (combined_wz + 1 + 1)* mword
+       h_index + (wz_fp + wz_f_index + 1 + 1) * mword *)
+    assert (next_hd_index == h_index_new1);
+    assert (Usize.v h_index_new1 <= heap_size);
+    wosize_times_mword_multiple_of_mword1 combined_wz_plus_one;
+    sum_of_multiple_of_mword_is_multiple_of_mword h_index (Usize.mul (Usize.add combined_wz_plus_one 1UL) mword);
+    if Usize.v h_index_new1 = heap_size then
+      (
+        ()
+      )
+    else
+    (
+        assert (is_hp_addr h_index_new1);
+        let f' =  objects2 h_index_new1 g1 in 
+        objects2_non_empty_lemma h_index_new1 g g1 fp f_index;
+        assert (Seq.length (objects2 h_index_new1 g1) > 0);
+        ()
+    )
+  )
+
+#restart-solver
+
+#restart-solver
+
+#restart-solver
+
+#restart-solver
+
+
+let objects2_singleton_lemma_test (h_index: hp_addr)
+                                  (g:heap)
+                         
+           : Lemma 
+            (ensures (Seq.length (objects2 h_index g) > 0 /\ 
+                        Usize.v (Usize.add h_index (Usize.mul (Usize.add (getWosize (read_word g h_index)) 1UL) mword)) == heap_size ==> 
+                          Seq.length (objects2 h_index g) == 1)) =
+  ()
+
+
+let objects2_singleton_lemma (h_index: hp_addr)
+                             (g:heap) 
+                      : Lemma 
+                        (requires (Seq.length (objects2 h_index g) > 0 /\
+                                   (Usize.v (Usize.add h_index (Usize.mul (Usize.add (getWosize (read_word g h_index)) 1UL) mword)) == heap_size)))
+                        (ensures (objects2 h_index g == Seq.create 1 h_index)) =
+ ()
+
+let cons_lemma (#a:eqtype)
+               (x:a)
+               (s:seq a)
+               (s1: seq a)
+    : Lemma
+      (requires length s > 0 /\ length s1 > 0 /\
+                (forall y. mem y s1 ==> mem y s))
+      (ensures (forall y. mem y (cons x s1) ==> mem y (cons x s))) =
+  assert (Seq.mem x (cons x s1));
+  assert (Seq.mem x (cons x s));
+  lemma_tl x s1;
+  lemma_tl x s;
+  ()
+                
+                
+#restart-solver
+
+#restart-solver
+
+#restart-solver
+
+#restart-solver
+
+#restart-solver
+
+#restart-solver
+
+#restart-solver
+
+#restart-solver
+
+#restart-solver
+
+#restart-solver
+
+let rec objects2_sub_set_lemma (h_index: hp_addr)
+                                 (g:heap) 
+                                 (g1:heap)
+                                 (fp:hp_addr{Usize.v fp >= Usize.v mword})
+                                 (f_index:hp_addr{Usize.v f_index >= Usize.v mword
+                                                  })
+                : Lemma
+                  (requires ( (* length of obj set of g > 0*)
+                              Seq.length (objects2 h_index g) > 0 /\
+                              (Seq.length (objects2 h_index g1) > 0) /\
+                              
+
+                              (* heap differs only in header of fp between g and g1*)
+                              heap_remains_same_except_index_v_id1 (hd_address fp) g g1 /\
+                             
+                              
+                             ((* header of f_index*)
+                              let hd_index = hd_address f_index in
+
+                              (* wosize of f_index in g*)
+                              let wz = getWosize (read_word g hd_index) in
+                              
+                              (* header of fp*)
+                              let hd_fp = hd_address fp in
+
+                              (*wosize of fp in g *)
+                              let cur_wosize = getWosize (read_word g hd_fp) in
+
+                              (* wosize of f_index and wosize of fp together*)
+                              let combined_wz = Usize.add cur_wosize wz in
+
+                              (* the combined wosize + 1 will be the coalesced wosize, so that now f_index header is also a field 
+                                 of fp after coalescing*)
+                              let combined_wz_plus_one = Usize.add combined_wz 1UL in
+
+                               (*The new wosize added to header of fp resulted into the new heap g1*)
+                               (* Therefore, new wosize of hd_fp in g1 is combined wosize + 1 *)
+                              ((getWosize (read_word g1 hd_fp) == combined_wz_plus_one) /\
+                                 
+                                 (* the header of f_index is the next header of fp in g*)
+                                 hd_index == Usize.add hd_fp (Usize.mul (Usize.add cur_wosize 1UL) mword) /\
+
+                                 
+                                Usize.v combined_wz_plus_one < heap_size /\
+
+                                (* The next header of f_index can be <= heap_size*)
+                                Usize.v (Usize.add hd_index (Usize.mul (Usize.add wz 1UL) mword)) <= heap_size)))
+                               )
+                  (ensures  (forall x. Seq.mem x (objects2 h_index g1) ==> Seq.mem x (objects2 h_index g)))
+                  (decreases (heap_size - Usize.v h_index)) =
+ let wz =  getWosize (read_word g h_index) in
+  let h_index_new =  Usize.add h_index (Usize.mul (Usize.add wz 1UL) mword) in
+  
+  wosize_times_mword_multiple_of_mword1 wz;
+  sum_of_multiple_of_mword_is_multiple_of_mword h_index (Usize.mul (Usize.add wz 1UL) mword);
+
+  let wz1 =  getWosize (read_word g1 h_index) in
+  let hd_fp = hd_address fp in
+  if h_index <> hd_fp then
+  (
+    assert (heap_remains_same_except_index_v_id1 (hd_address fp) g g1);
+    assert (wz == wz1);
+    assert (Usize.v wz <> 0);
+    if Usize.v h_index_new <= heap_size then
+    (
+      if Usize.v h_index_new = heap_size then
+      (
+        let f = Seq.create 1 h_index in
+        objects2_singleton_lemma h_index g;
+        assert (objects2 h_index g == Seq.create 1 h_index);
+        assert (objects2 h_index g1 == Seq.create 1 h_index);
+        assert (forall x. Seq.mem x (objects2 h_index g1) ==> Seq.mem x (objects2 h_index g));
+        ()
+      )
+      else
+      (
+        assert (is_hp_addr h_index_new);
+        let f' =  objects2 h_index_new g1 in
+        let f1 =  objects2 h_index_new g in
+        objects2_sub_set_lemma h_index_new g g1 fp f_index;
+        assert (forall x. Seq.mem x (objects2 h_index_new g1) ==> Seq.mem x (objects2 h_index_new g));
+        assert (Seq.length f' > 0);
+        lemma_tl h_index f';
+        let f'' = cons h_index f' in
+
+        lemma_tl h_index f1;
+        let f2 = cons h_index f1 in
+        assert (f'' == objects2 h_index g1);
+        assert (f2 == objects2 h_index g);
+        assert (forall x. Seq.mem x f'' ==> Seq.mem x f2);
+        cons_lemma h_index f2 f'';
+        assert (forall x. Seq.mem x (objects2 h_index g1) ==> Seq.mem x (objects2 h_index g));
+        (*objects2_non_empty_lemma h_index_new g g1 fp f_index;
+        assert (Seq.length (objects2 h_index_new g1) > 0);
+        ()*)
+        ()
+      )
+    )
+    else
+    (
+      ()
+    )
+  )
+  else
+  (
+    assert (h_index == hd_fp);
+    let hd_index = hd_address f_index in
+    let wz_f_index = getWosize (read_word g hd_index) in
+    let hd_fp = hd_address fp in
+    let cur_wosize = getWosize (read_word g hd_fp) in
+    let combined_wz = Usize.add cur_wosize wz_f_index in
+    let combined_wz_plus_one = Usize.add combined_wz 1UL in
+    let new_fp_wosize = getWosize (read_word g1 hd_fp) in
+    assert (new_fp_wosize == combined_wz_plus_one);
+    assert (Usize.v combined_wz_plus_one > 0);
+    let h_index_new1 = Usize.add h_index (Usize.mul (Usize.add combined_wz_plus_one 1UL) mword) in
+    assert (Usize.v combined_wz_plus_one < heap_size);
+    let next_hd_index = Usize.add hd_index (Usize.mul (Usize.add wz_f_index 1UL) mword) in
+    (* h_index + (combined_wz_plus_one + 1) * mword
+       h_index + (combined_wz + 1 + 1)* mword
+       h_index + (wz_fp + wz_f_index + 1 + 1) * mword *)
+    assert (next_hd_index == h_index_new1);
+    assert (Usize.v h_index_new1 <= heap_size);
+    wosize_times_mword_multiple_of_mword1 combined_wz_plus_one;
+    sum_of_multiple_of_mword_is_multiple_of_mword h_index (Usize.mul (Usize.add combined_wz_plus_one 1UL) mword);
+    if Usize.v h_index_new1 = heap_size then
+      (
+        objects2_singleton_lemma h_index g1;
+        assert (Usize.v h_index_new < heap_size);
+        assert (h_index_new1 == Usize.add h_index_new (Usize.mul (Usize.add (getWosize (read_word g h_index_new)) 1UL) mword));
+        assert (forall x. Seq.mem x (objects2 h_index g1) ==> Seq.mem x (objects2 h_index g));
+        ()
+      )
+    else
+    (
+        assert (is_hp_addr h_index_new1);
+        let f' =  objects2 h_index_new1 g1 in 
+        objects2_sub_set_lemma h_index_new1 g g1 fp f_index;
+        
+        assert (forall x. Seq.mem x (objects2 h_index_new1 g1) ==> Seq.mem x (objects2 h_index_new1 g));
+        lemma_tl h_index f';
+        let f'' = cons h_index f' in
+
+        let f1 = objects2 h_index_new1 g in 
+        
+        lemma_tl h_index_new f1;
+        let f2 = cons h_index_new f1 in
+
+        lemma_tl h_index f2;
+        let f3 = cons h_index f2 in
+        
+        assert (forall x. Seq.mem x f2 ==> Seq.mem x f3);
+        assert (forall x. Seq.mem x f1 ==> Seq.mem x f2);
+
+        assert (forall x. Seq.mem x f' ==> Seq.mem x f1);
+        assert (forall x. Seq.mem x f' ==> Seq.mem x f'');
+        assert (forall x. Seq.mem x f'' ==> Seq.mem x f3);
+        
+        ()
+    )
+  )
+ 
+#restart-solver
+
+#restart-solver
+
+#restart-solver
+
+#restart-solver
+
+#restart-solver
+
+#restart-solver
+
+#restart-solver
+
+#restart-solver
+
+#restart-solver
+
+#restart-solver
+
+#restart-solver
+
+let rec objects2_mem_coalescing_lemma (h_index: hp_addr)
+                                 (g:heap) 
+                                 (g1:heap)
+                                 (fp:hp_addr{Usize.v fp >= Usize.v mword})
+                                 (f_index:hp_addr{Usize.v f_index >= Usize.v mword
+                                                  })
+                : Lemma
+                  (requires ( (* length of obj set of g > 0*)
+                              Seq.length (objects2 h_index g) > 0 /\
+                              (Seq.length (objects2 h_index g1) > 0) /\
+                              
+                              (* heap differs only in header of fp between g and g1*)
+                              heap_remains_same_except_index_v_id1 (hd_address fp) g g1 /\
+                             
+                              
+                             ((* header of f_index*)
+                              let hd_index = hd_address f_index in
+
+                              (* wosize of f_index in g*)
+                              let wz = getWosize (read_word g hd_index) in
+                              
+                              (* header of fp*)
+                              let hd_fp = hd_address fp in
+
+                              (*wosize of fp in g *)
+                              let cur_wosize = getWosize (read_word g hd_fp) in
+
+                              (* wosize of f_index and wosize of fp together*)
+                              let combined_wz = Usize.add cur_wosize wz in
+
+                              (* the combined wosize + 1 will be the coalesced wosize, so that now f_index header is also a field 
+                                 of fp after coalescing*)
+                              let combined_wz_plus_one = Usize.add combined_wz 1UL in
+
+                               (*The new wosize added to header of fp resulted into the new heap g1*)
+                               (* Therefore, new wosize of hd_fp in g1 is combined wosize + 1 *)
+                              ((getWosize (read_word g1 hd_fp) == combined_wz_plus_one) /\
+                                 
+                                 (* the header of f_index is the next header of fp in g*)
+                                 hd_index == Usize.add hd_fp (Usize.mul (Usize.add cur_wosize 1UL) mword) /\
+
+                                 
+                                Usize.v combined_wz_plus_one < heap_size /\
+
+                                (* The next header of f_index can be <= heap_size*)
+                                Usize.v (Usize.add hd_index (Usize.mul (Usize.add wz 1UL) mword)) <= heap_size)))
+                               )
+                  (ensures (forall x. Seq.mem x (objects2 h_index g) /\ x <> (hd_address f_index) ==>
+                                      Seq.mem x (objects2 h_index g1)))
+                  (decreases (heap_size - Usize.v h_index)) =
+  let wz =  getWosize (read_word g h_index) in
+  let h_index_new =  Usize.add h_index (Usize.mul (Usize.add wz 1UL) mword) in
+  
+  wosize_times_mword_multiple_of_mword1 wz;
+  sum_of_multiple_of_mword_is_multiple_of_mword h_index (Usize.mul (Usize.add wz 1UL) mword);
+
+  let wz1 =  getWosize (read_word g1 h_index) in
+  let hd_fp = hd_address fp in
+  if h_index <> hd_fp then
+  (
+    assert (heap_remains_same_except_index_v_id1 (hd_address fp) g g1);
+    assert (wz == wz1);
+    assert (Usize.v wz <> 0);
+   
+      if Usize.v h_index_new = heap_size then
+      (
+        let f = Seq.create 1 h_index in
+        objects2_singleton_lemma h_index g;
+        assert (objects2 h_index g == Seq.create 1 h_index);
+        assert (objects2 h_index g1 == Seq.create 1 h_index);
+        assert (forall x. Seq.mem x (objects2 h_index g) /\ x <> (hd_address f_index) ==>
+                                      Seq.mem x (objects2 h_index g1));
+        ()
+      )
+      else
+      (
+        assert (is_hp_addr h_index_new);
+        let f' =  objects2 h_index_new g1 in
+        let f1 =  objects2 h_index_new g in
+        objects2_mem_coalescing_lemma h_index_new g g1 fp f_index;
+        assert (forall x. Seq.mem x (objects2 h_index_new g) /\ x <> (hd_address f_index) ==>
+                                      Seq.mem x (objects2 h_index_new g1));
+        assert (Seq.length f' > 0);
+        lemma_tl h_index f';
+        let f'' = cons h_index f' in
+
+        lemma_tl h_index f1;
+        let f2 = cons h_index f1 in
+        assert (f'' == objects2 h_index g1);
+        assert (f2 == objects2 h_index g);
+        
+        //cons_lemma h_index f2 f'';
+        assert (forall x. Seq.mem x (objects2 h_index g) /\ x <> (hd_address f_index) ==>
+                                      Seq.mem x (objects2 h_index g1));
+        ()
+      )
+    )
+else
+(
+  assert (h_index == hd_fp);
+    let hd_index = hd_address f_index in
+    let wz_f_index = getWosize (read_word g hd_index) in
+    let hd_fp = hd_address fp in
+    let cur_wosize = getWosize (read_word g hd_fp) in
+    let combined_wz = Usize.add cur_wosize wz_f_index in
+    let combined_wz_plus_one = Usize.add combined_wz 1UL in
+    let new_fp_wosize = getWosize (read_word g1 hd_fp) in
+    assert (new_fp_wosize == combined_wz_plus_one);
+    assert (Usize.v combined_wz_plus_one > 0);
+    let h_index_new1 = Usize.add h_index (Usize.mul (Usize.add combined_wz_plus_one 1UL) mword) in
+    assert (Usize.v combined_wz_plus_one < heap_size);
+    let next_hd_index = Usize.add hd_index (Usize.mul (Usize.add wz_f_index 1UL) mword) in
+    assert (next_hd_index == h_index_new1);
+    assert (Usize.v h_index_new1 <= heap_size);
+    wosize_times_mword_multiple_of_mword1 combined_wz_plus_one;
+    sum_of_multiple_of_mword_is_multiple_of_mword h_index (Usize.mul (Usize.add combined_wz_plus_one 1UL) mword);
+    if Usize.v h_index_new1 = heap_size then
+      (
+        objects2_singleton_lemma h_index g1;
+        assert (Usize.v h_index_new < heap_size);
+        assert (forall x. Seq.mem x (objects2 h_index g) /\ x <> (hd_address f_index) ==>
+                                      Seq.mem x (objects2 h_index g1));
+        ()
+      )
+    else
+     (
+        assert (is_hp_addr h_index_new1);
+        let f' =  objects2 h_index_new1 g1 in 
+        objects2_mem_coalescing_lemma h_index_new1 g g1 fp f_index;
+        
+        assert (forall x. Seq.mem x (objects2 h_index_new1 g) /\ x <> (hd_address f_index) ==>
+                                      Seq.mem x (objects2 h_index_new1 g1));
+
+        lemma_tl h_index f';
+        let f'' = cons h_index f' in
+
+        let f1 = objects2 h_index_new1 g in 
+        
+        lemma_tl h_index_new f1;
+        let f2 = cons h_index_new f1 in
+
+        lemma_tl h_index f2;
+        let f3 = cons h_index f2 in
+        assert (forall x. Seq.mem x (objects2 h_index g) /\ x <> (hd_address f_index) ==>
+                                      Seq.mem x (objects2 h_index g1));
+       ()
+     )
+)
+  
+let wosize_plus_times_mword_multiple_of_mword (wz:wosize)
+                     :Lemma 
+                      (ensures (Usize.v (Usize.mul (Usize.add wz 1UL) mword) % Usize.v mword == 0)) = ()
+
+let rec objects2_interval_lemma (h_index: hp_addr)
+                                (g:heap) 
+                : Lemma
+                  (requires True)
+                  (ensures (Seq.length (objects2 h_index g) > 0 ==>
+                              (forall x y. Seq.mem x (objects2 h_index g) /\ 
+                                                   (Usize.v y > Usize.v x) /\ 
+                                                   (Usize.v y <= Usize.v x + (((Usize.v (getWosize (read_word g x)) + 1) * Usize.v mword) - 1)) ==>
+                                                   ~(Seq.mem y (objects2 h_index g)))))
+                   (decreases (heap_size - Usize.v h_index)) =
+let wz =  getWosize (read_word g h_index) in
+let h_index_new =  Usize.add h_index (Usize.mul (Usize.add wz 1UL) mword) in
+if Usize.v wz = 0 then 
+(
+  ()
+)
+else
+(
+  let h_index_new =  Usize.add h_index (Usize.mul (Usize.add wz 1UL) mword) in // possible next header = h_index + (wz + 1) * mword. Eg. h_index = 0; wz = 1; mword = 8;
+                                                                               // h_index_new = 0 + (1 + 1) * 8 = 0 + 16 = 16. h_index range in g = 0......7
+                                                                               // first field range in g = 8......15. Only one field. So next header starts at 16
+  if Usize.v h_index_new <= heap_size then
+  (
+    if Usize.v h_index_new = heap_size then // h_index_new == heap_size --> The last block is h_index, So just create a singleton with h_index and return.
+    (
+      ()
+    )
+    else
+    (
+      wosize_plus_times_mword_multiple_of_mword wz;
+      sum_of_multiple_of_mword_is_multiple_of_mword h_index (Usize.mul (Usize.add wz 1UL) mword);
+      assert (Usize.v h_index_new % Usize.v mword == 0);
+      assert (is_hp_addr h_index_new);
+      let f' =  objects2 h_index_new g in
+      objects2_interval_lemma h_index_new g;
+      if length f' = 0 then 
+      (
+        ()
+      )
+      else
+      (
+         lemma_tl h_index f';
+         let f'' = cons h_index f' in
+         ()
+      )
+    )
+  )
+  else
+  (
+    ()
+  )
+)
+
+let objects2_non_mem_lemma (h_index: hp_addr)
+                           (g:heap)
+          : Lemma 
+            (requires (Seq.length (objects2 0UL g) > 0 /\
+                       Seq.mem h_index (objects2 0UL g)))
+            
+            (ensures (let wz = getWosize (read_word g h_index) in
+                      let h_index_new = Usize.add h_index (Usize.mul (Usize.add wz 1UL) mword) in
+                       ~(exists x. Seq.mem x (objects2 0UL g) /\ Usize.v x > Usize.v h_index /\
+                                                     Usize.v x < Usize.v h_index_new))) =
+  let wz = getWosize (read_word g h_index) in
+  let h_index_new = Usize.add h_index (Usize.mul (Usize.add wz 1UL) mword) in
+  let obj = objects2 0UL g in
+  objects2_interval_lemma 0UL g;
+
+  assert (forall x y. Seq.mem x obj /\ 
+                      (Usize.v y > Usize.v x) /\ 
+                      (Usize.v y <= Usize.v x + (((Usize.v (getWosize (read_word g x)) + 1) * Usize.v mword) - 1)) ==>
+                                          ~(Seq.mem y obj));
+  
+  assert (Seq.mem h_index (objects2 0UL g));
+  
+  assert (forall y. 
+                      (Usize.v y > Usize.v h_index) /\ 
+                      (Usize.v y <= Usize.v h_index + (((Usize.v (getWosize (read_word g h_index)) + 1) * Usize.v mword) - 1)) ==>
+                                          ~(Seq.mem y obj));
+  assert (forall y. 
+                      (Usize.v y > Usize.v h_index) /\ 
+                      (Usize.v y <= Usize.v h_index_new - 1) ==>
+                                          ~(Seq.mem y obj));
+  
+  assert (forall y. 
+                      (Usize.v y > Usize.v h_index) /\ 
+                      (Usize.v y < Usize.v h_index_new) ==>
+                                          ~(Seq.mem y obj));
+  
+  assert (~(exists x. Seq.mem x (objects2 0UL g) /\ Usize.v x > Usize.v h_index /\
+                                                     Usize.v x < Usize.v h_index_new));
+  ()
+
+
+#restart-solver
+
+let objects2_non_mem_lemma2 (h_index: hp_addr)
+                            (g:heap)
+          : Lemma 
+            (requires True)
+            
+            (ensures ((Seq.length (objects2 0UL g) > 0 /\
+                       Seq.mem h_index (objects2 0UL g)) ==>
+                      (let wz = getWosize (read_word g h_index) in
+                      let h_index_new = Usize.add h_index (Usize.mul (Usize.add wz 1UL) mword) in
+                       ~(exists x. Seq.mem x (objects2 0UL g) /\ Usize.v x > Usize.v h_index /\
+                                                     Usize.v x < Usize.v h_index_new)))) =
+  let wz = getWosize (read_word g h_index) in
+  let h_index_new = Usize.add h_index (Usize.mul (Usize.add wz 1UL) mword) in
+  let obj = objects2 0UL g in
+  objects2_interval_lemma 0UL g;
+  ()
+
+
+            
+
+
+
+                      
 let objects2_mem_lemma (h_index: hp_addr)
                            (g:heap)
-
-
-          : Lemma
+                           
+                      
+          : Lemma 
             (ensures (let wz =  getWosize (read_word g h_index) in
                       let h_index_new =  Usize.add h_index (Usize.mul (Usize.add wz 1UL) mword) in
                       (Seq.length (objects2 h_index g) > 0 /\ (Usize.v h_index_new < heap_size) ==> Seq.mem h_index_new (objects2 h_index g))))
-            (decreases (heap_size - Usize.v h_index)) =
+            (decreases (heap_size - Usize.v h_index)) = 
 let wz =  getWosize (read_word g h_index) in
 let h_index_new =  Usize.add h_index (Usize.mul (Usize.add wz 1UL) mword) in
-if Usize.v wz = 0 then
+if Usize.v wz = 0 then 
 (
   let f' = Seq.empty  in// There are no zero length objects.
   assert (Seq.length f' > 0 /\ (Usize.v h_index_new < heap_size) ==> Seq.mem h_index_new f');
@@ -374,7 +1103,7 @@ else
     (
        assert (Usize.v h_index_new == heap_size);
        let f = Seq.create 1 h_index in
-
+       
        G.is_vertex_set_lemma2 f;
        assert (Seq.length f > 0 /\ (Usize.v h_index_new < heap_size) ==> Seq.mem h_index_new f);
        ()
@@ -386,18 +1115,18 @@ else
       sum_of_multiple_of_mword_is_multiple_of_mword h_index (Usize.mul (Usize.add wz 1UL) mword);
       assert (Usize.v h_index_new % Usize.v mword == 0);
       assert (is_hp_addr h_index_new);
-      let f' =  objects2 h_index_new g in
-      if length f' = 0 then
+      let f' =  objects2 h_index_new g in 
+      if length f' = 0 then 
       (
         assert (Seq.length f' > 0 /\ (Usize.v h_index_new < heap_size) ==> Seq.mem h_index_new f');
         ()
       )
        else
        (
-
+        
          lemma_tl h_index f';
          let f'' = cons h_index f' in
-
+         
          G.is_vertex_set_cons h_index f';
          assert (Seq.length f'' > 0 /\ (Usize.v h_index_new < heap_size) ==> Seq.mem h_index_new f'');
          ()
@@ -413,28 +1142,28 @@ else
   )
 )
 
-#restart-solver
+#restart-solver 
 
-#restart-solver
+#restart-solver 
 
 let rec objects2_mem_lemma1 (h_index: hp_addr)
                             (g:heap)
-
-
-          : Lemma
-            (ensures ((Seq.length (objects2 h_index g) > 0  ==> (forall x. Seq.mem x (objects2 h_index g) /\
-                                                                  Usize.v (Usize.add x (Usize.mul (Usize.add (getWosize (read_word g x)) 1UL) mword)) < heap_size ==>
-                                                                       Seq.mem (Usize.add x (Usize.mul (Usize.add (getWosize (read_word g x)) 1UL) mword))
+                           
+                      
+          : Lemma 
+            (ensures ((Seq.length (objects2 h_index g) > 0  ==> (forall x. Seq.mem x (objects2 h_index g) /\ 
+                                                                  Usize.v (Usize.add x (Usize.mul (Usize.add (getWosize (read_word g x)) 1UL) mword)) < heap_size ==> 
+                                                                       Seq.mem (Usize.add x (Usize.mul (Usize.add (getWosize (read_word g x)) 1UL) mword)) 
                                                                            (objects2 h_index g))))) =
 let wz =  getWosize (read_word g h_index) in
 let h_index_new =  Usize.add h_index (Usize.mul (Usize.add wz 1UL) mword) in
-if Usize.v wz = 0 then
+if Usize.v wz = 0 then 
 (
   let f' = Seq.empty  in// There are no zero length objects.
   assert (Seq.length f' > 0 /\ (Usize.v h_index_new < heap_size) ==> Seq.mem h_index_new f');
-  assert (Seq.length (objects2 h_index g) > 0  ==> (forall x. Seq.mem x (objects2 h_index g) /\
-                                                                  Usize.v (Usize.add x (Usize.mul (Usize.add (getWosize (read_word g x)) 1UL) mword)) < heap_size ==>
-                                                                       Seq.mem (Usize.add x (Usize.mul (Usize.add (getWosize (read_word g x)) 1UL) mword))
+  assert (Seq.length (objects2 h_index g) > 0  ==> (forall x. Seq.mem x (objects2 h_index g) /\ 
+                                                                  Usize.v (Usize.add x (Usize.mul (Usize.add (getWosize (read_word g x)) 1UL) mword)) < heap_size ==> 
+                                                                       Seq.mem (Usize.add x (Usize.mul (Usize.add (getWosize (read_word g x)) 1UL) mword)) 
                                                                            (objects2 h_index g)));
   ()
 )
@@ -449,12 +1178,12 @@ else
     (
        assert (Usize.v h_index_new == heap_size);
        let f = Seq.create 1 h_index in
-
+       
        G.is_vertex_set_lemma2 f;
        assert (Seq.length f > 0 /\ (Usize.v h_index_new < heap_size) ==> Seq.mem h_index_new f);
-       assert (Seq.length (objects2 h_index g) > 0  ==> (forall x. Seq.mem x (objects2 h_index g) /\
-                                                                  Usize.v (Usize.add x (Usize.mul (Usize.add (getWosize (read_word g x)) 1UL) mword)) < heap_size ==>
-                                                                       Seq.mem (Usize.add x (Usize.mul (Usize.add (getWosize (read_word g x)) 1UL) mword))
+       assert (Seq.length (objects2 h_index g) > 0  ==> (forall x. Seq.mem x (objects2 h_index g) /\ 
+                                                                  Usize.v (Usize.add x (Usize.mul (Usize.add (getWosize (read_word g x)) 1UL) mword)) < heap_size ==> 
+                                                                       Seq.mem (Usize.add x (Usize.mul (Usize.add (getWosize (read_word g x)) 1UL) mword)) 
                                                                            (objects2 h_index g)));
        ()
     )
@@ -467,12 +1196,12 @@ else
       assert (is_hp_addr h_index_new);
       let f' =  objects2 h_index_new g in
       objects2_mem_lemma1 h_index_new g;
-      if length f' = 0 then
+      if length f' = 0 then 
       (
         assert (Seq.length f' > 0 /\ (Usize.v h_index_new < heap_size) ==> Seq.mem h_index_new f');
-        assert (Seq.length (objects2 h_index g) > 0  ==> (forall x. Seq.mem x (objects2 h_index g) /\
-                                                                  Usize.v (Usize.add x (Usize.mul (Usize.add (getWosize (read_word g x)) 1UL) mword)) < heap_size ==>
-                                                                       Seq.mem (Usize.add x (Usize.mul (Usize.add (getWosize (read_word g x)) 1UL) mword))
+        assert (Seq.length (objects2 h_index g) > 0  ==> (forall x. Seq.mem x (objects2 h_index g) /\ 
+                                                                  Usize.v (Usize.add x (Usize.mul (Usize.add (getWosize (read_word g x)) 1UL) mword)) < heap_size ==> 
+                                                                       Seq.mem (Usize.add x (Usize.mul (Usize.add (getWosize (read_word g x)) 1UL) mword)) 
                                                                            (objects2 h_index g)));
         ()
       )
@@ -483,9 +1212,9 @@ else
          assert (Seq.length f'' > 0 /\ (Usize.v h_index_new < heap_size) ==> Seq.mem h_index_new f'');
          G.is_vertex_set_cons h_index f';
          assert (Seq.length f'' > 0 /\ (Usize.v h_index_new < heap_size) ==> Seq.mem h_index_new f'');
-         assert (Seq.length (objects2 h_index g) > 0  ==> (forall x. Seq.mem x (objects2 h_index g) /\
-                                                                  Usize.v (Usize.add x (Usize.mul (Usize.add (getWosize (read_word g x)) 1UL) mword)) < heap_size ==>
-                                                                       Seq.mem (Usize.add x (Usize.mul (Usize.add (getWosize (read_word g x)) 1UL) mword))
+         assert (Seq.length (objects2 h_index g) > 0  ==> (forall x. Seq.mem x (objects2 h_index g) /\ 
+                                                                  Usize.v (Usize.add x (Usize.mul (Usize.add (getWosize (read_word g x)) 1UL) mword)) < heap_size ==> 
+                                                                       Seq.mem (Usize.add x (Usize.mul (Usize.add (getWosize (read_word g x)) 1UL) mword)) 
                                                                            (objects2 h_index g)));
          ()
        )
@@ -496,13 +1225,71 @@ else
     assert (Usize.v h_index_new > heap_size); //h_index_new is greater than heap_size means the last object size exceeds the heap.
     let f' = Seq.empty in
     assert (Seq.length f' > 0 /\ (Usize.v h_index_new < heap_size) ==> Seq.mem h_index_new f');
-    assert (Seq.length (objects2 h_index g) > 0  ==> (forall x. Seq.mem x (objects2 h_index g) /\
-                                                                  Usize.v (Usize.add x (Usize.mul (Usize.add (getWosize (read_word g x)) 1UL) mword)) < heap_size ==>
-                                                                       Seq.mem (Usize.add x (Usize.mul (Usize.add (getWosize (read_word g x)) 1UL) mword))
+    assert (Seq.length (objects2 h_index g) > 0  ==> (forall x. Seq.mem x (objects2 h_index g) /\ 
+                                                                  Usize.v (Usize.add x (Usize.mul (Usize.add (getWosize (read_word g x)) 1UL) mword)) < heap_size ==> 
+                                                                       Seq.mem (Usize.add x (Usize.mul (Usize.add (getWosize (read_word g x)) 1UL) mword)) 
                                                                            (objects2 h_index g)));
     ()
   )
 )
+
+#restart-solver
+
+#restart-solver
+
+let rec objects2_interval_lemma (h_index: hp_addr)
+                                (g:heap) 
+                : Lemma
+                  (requires True)
+                  (ensures (Seq.length (objects2 h_index g) > 0 ==>
+                              (forall x y. Seq.mem x (objects2 h_index g) /\ 
+                                                   (Usize.v y > Usize.v x) /\ 
+                                                   (Usize.v y <= Usize.v x + (((Usize.v (getWosize (read_word g x)) + 1) * Usize.v mword) - 1)) ==>
+                                                   ~(Seq.mem y (objects2 h_index g)))))
+                   (decreases (heap_size - Usize.v h_index)) =
+let wz =  getWosize (read_word g h_index) in
+let h_index_new =  Usize.add h_index (Usize.mul (Usize.add wz 1UL) mword) in
+if Usize.v wz = 0 then 
+(
+  ()
+)
+else
+(
+  let h_index_new =  Usize.add h_index (Usize.mul (Usize.add wz 1UL) mword) in // possible next header = h_index + (wz + 1) * mword. Eg. h_index = 0; wz = 1; mword = 8;
+                                                                               // h_index_new = 0 + (1 + 1) * 8 = 0 + 16 = 16. h_index range in g = 0......7
+                                                                               // first field range in g = 8......15. Only one field. So next header starts at 16
+  if Usize.v h_index_new <= heap_size then
+  (
+    if Usize.v h_index_new = heap_size then // h_index_new == heap_size --> The last block is h_index, So just create a singleton with h_index and return.
+    (
+      ()
+    )
+    else
+    (
+      wosize_plus_times_mword_multiple_of_mword wz;
+      sum_of_multiple_of_mword_is_multiple_of_mword h_index (Usize.mul (Usize.add wz 1UL) mword);
+      assert (Usize.v h_index_new % Usize.v mword == 0);
+      assert (is_hp_addr h_index_new);
+      let f' =  objects2 h_index_new g in
+      objects2_interval_lemma h_index_new g;
+      if length f' = 0 then 
+      (
+        ()
+      )
+      else
+      (
+         lemma_tl h_index f';
+         let f'' = cons h_index f' in
+         ()
+      )
+    )
+  )
+  else
+  (
+    ()
+  )
+)
+
 
 (*assume (Usize.v f_index_new >= heap_size ==> ~(Seq.mem h_index_new (objects2 h_index g)))*)
 
@@ -521,14 +1308,14 @@ else
     (
        assert (Usize.v h_index_new == heap_size);
        let f = Seq.create 1 h_index in
-
+       
        G.is_vertex_set_lemma2 f;
        ()
     )
     else
     (
       assert (Usize.v h_index_new < heap_size); // h_index_new < heap_size, still more blocks to explore, hence recurse.
-      let f' =  objects2 h_index_new g in
+      let f' =  objects2 h_index_new g in 
       objects2_equal_lemma h_index_new g g';
       if length f' = 0 then ()
        else
@@ -536,13 +1323,13 @@ else
          (*lemma_tail_snoc f' h_index;
          lemma_mem_snoc f' h_index;
          let f'' = snoc f' h_index in
-
+         
          G.snoc_unique_lemma h_index f';*)
          lemma_tl h_index f';
          let f'' = cons h_index f' in
          assert (Seq.length f'' > 0 /\ (Usize.v h_index_new < heap_size) ==> Seq.mem h_index_new f'');
          G.is_vertex_set_cons h_index f';
-
+         
          ()
        )
     )
@@ -555,7 +1342,7 @@ else
 )
 
 let wosize_times_mword_multiple_of_mword5 (wz:wosize)
-                     :Lemma
+                     :Lemma 
                       (ensures (Usize.v (Usize.mul (Usize.add wz 1UL)  mword) % Usize.v mword == 0)) = ()
 
 
@@ -565,13 +1352,13 @@ let wosize_times_mword_multiple_of_mword5 (wz:wosize)
 
 let objects2_mem_lemma1_app3 (h_index: hp_addr)
                             (g:heap)
-
-
-          : Lemma
-            (requires (Seq.length (objects2 0UL g) > 0 /\ Seq.mem h_index (objects2 0UL g) /\
+                           
+                      
+          : Lemma 
+            (requires (Seq.length (objects2 0UL g) > 0 /\ Seq.mem h_index (objects2 0UL g) /\ 
                         Usize.v (Usize.add h_index (Usize.mul (Usize.add (getWosize (read_word g h_index)) 1UL) mword)) < heap_size))
-            (ensures (Seq.mem (Usize.add h_index (Usize.mul (Usize.add (getWosize (read_word g h_index)) 1UL) mword)) (objects2 0UL g))) =
-
+            (ensures (Seq.mem (Usize.add h_index (Usize.mul (Usize.add (getWosize (read_word g h_index)) 1UL) mword)) (objects2 0UL g))) = 
+  
   let s = objects2 0UL g in
   objects2_mem_lemma1 0UL g;
   let h_index_new = Usize.add h_index (Usize.mul (Usize.add (getWosize (read_word g h_index)) 1UL) mword) in
@@ -579,13 +1366,13 @@ let objects2_mem_lemma1_app3 (h_index: hp_addr)
   assert (Seq.mem h_index_new s);
   ()
 
-#restart-solver
+#restart-solver 
 
-#restart-solver
+#restart-solver 
 
-let rec objects2_equal_lemma3 (h_index:hp_addr)
-                          (g:heap)
-                          (g':heap)
+let rec objects2_equal_lemma3 (h_index:hp_addr) 
+                          (g:heap) 
+                          (g':heap) 
                    : Lemma
                        (requires (objects2 0UL g == objects2 0UL g') /\
                                  (Seq.mem h_index (objects2 0UL g)) /\
@@ -601,10 +1388,10 @@ else
   let h_index_new =  Usize.add h_index (Usize.mul (Usize.add wz 1UL) mword) in // possible next header = h_index + (wz + 1) * mword. Eg. h_index = 0; wz = 1; mword = 8;
   wosize_times_mword_multiple_of_mword wz;
   assert (Usize.v (Usize.mul (Usize.add wz 1UL) mword) % Usize.v mword == 0);
-
-  sum_of_multiple_of_mword_is_multiple_of_mword h_index (Usize.mul (Usize.add wz 1UL) mword);                                                                             // h_index_new = 0 +
+  
+  sum_of_multiple_of_mword_is_multiple_of_mword h_index (Usize.mul (Usize.add wz 1UL) mword);                                                                             // h_index_new = 0 + 
                                                                       // first field range in g = 8......15. Only one field. So next header starts at 16
-  assert ((Usize.v h_index + Usize.v (Usize.mul (Usize.add wz 1UL) mword)) % Usize.v mword == 0);
+  assert ((Usize.v h_index + Usize.v (Usize.mul (Usize.add wz 1UL) mword)) % Usize.v mword == 0);                                                                    
   assert (Usize.v h_index_new % Usize.v mword == 0);
   if Usize.v h_index_new <= heap_size then //valid heap condition
   (
@@ -612,7 +1399,7 @@ else
     (
        assert (Usize.v h_index_new == heap_size);
        let f = Seq.create 1 h_index in
-
+       
        G.is_vertex_set_lemma2 f;
        ()
     )
@@ -620,7 +1407,7 @@ else
     (
       assert (Usize.v h_index_new < heap_size); // h_index_new < heap_size, still more blocks to explore, hence recurse.
       assert (is_hp_addr h_index_new);
-      let f' =  objects2 h_index_new g in
+      let f' =  objects2 h_index_new g in 
       objects2_mem_lemma1_app3 h_index g;
       assert (Seq.mem h_index_new (objects2 0UL g));
       objects2_equal_lemma3 h_index_new g g';
@@ -630,14 +1417,14 @@ else
          (*lemma_tail_snoc f' h_index;
          lemma_mem_snoc f' h_index;
          let f'' = snoc f' h_index in
-
+         
          G.snoc_unique_lemma h_index f';*)
          assert (Seq.mem h_index (objects2 0UL g));
          lemma_tl h_index f';
          let f'' = cons h_index f' in
          assert (Seq.length f'' > 0 /\ (Usize.v h_index_new < heap_size) ==> Seq.mem h_index_new f'');
          G.is_vertex_set_cons h_index f';
-
+         
          ()
        )
     )
@@ -649,7 +1436,7 @@ else
   )
 )
 
-#restart-solver
+#restart-solver 
 
 let rec objects2_length_lemma h_index g =
  let wz =  getWosize (read_word g h_index) in
@@ -666,14 +1453,14 @@ else
     (
        assert (Usize.v h_index_new == heap_size);
        let f = Seq.create 1 h_index in
-
+       
        G.is_vertex_set_lemma2 f;
        ()
     )
     else
     (
       assert (Usize.v h_index_new < heap_size); // h_index_new < heap_size, still more blocks to explore, hence recurse.
-      let f' =  objects2 h_index_new g in
+      let f' =  objects2 h_index_new g in 
       objects2_length_lemma h_index_new g;
       if length f' = 0 then ()
        else
@@ -681,7 +1468,7 @@ else
          (*lemma_tail_snoc f' h_index;
          lemma_mem_snoc f' h_index;
          let f'' = snoc f' h_index in
-
+         
          G.snoc_unique_lemma h_index f';*)
          lemma_tl h_index f';
          let f'' = cons h_index f' in
@@ -711,42 +1498,42 @@ else
    wosize_times_mword_multiple_of_mword wz;
   assert (Usize.v (Usize.mul wz mword) % Usize.v mword == 0);
 
-  sum_of_multiple_of_mword_is_multiple_of_mword h_index (Usize.mul wz mword);
+  sum_of_multiple_of_mword_is_multiple_of_mword h_index (Usize.mul wz mword);                                                                               
   if Usize.v h_index_new <= heap_size then //valid heap condition
-
+  
   (
     if Usize.v h_index_new = heap_size then // h_index_new == heap_size --> The last block is h_index, So just create a singleton with h_index and return.
     (
        assert (Usize.v h_index_new == heap_size);
        let f = Seq.create 1 h_index in
-
+       
        G.is_vertex_set_lemma2 f;
        ()
     )
     else
     (
       assert (Usize.v h_index_new < heap_size); // h_index_new < heap_size, still more blocks to explore, hence recurse.
-      let f' =  objects2 h_index_new g in
+      let f' =  objects2 h_index_new g in 
       objects2_color_lemma h_index_new g;
       assert ((forall x. Seq.mem x (objects2 h_index_new g) ==> color_of_object1 x g == white \/
                                                            color_of_object1 x g == gray \/
                                                            color_of_object1 x g == black \/
                                                            color_of_object1 x g == blue));
-      assert ((forall x. Seq.mem x f' ==> color_of_object1 x g == white \/
+      assert ((forall x. Seq.mem x f' ==> color_of_object1 x g == white \/ 
                                      color_of_object1 x g == gray \/
                                      color_of_object1 x g == black \/
                                      color_of_object1 x g == blue));
-      assert (color_of_object1 h_index g == white \/
+      assert (color_of_object1 h_index g == white \/ 
               color_of_object1 h_index g == gray \/
               color_of_object1 h_index g == black \/
-              color_of_object1 h_index g == blue);
+              color_of_object1 h_index g == blue);  
       if length f' = 0 then ()
        else
        (
          (*lemma_tail_snoc f' h_index;
          lemma_mem_snoc f' h_index;
          let f'' = snoc f' h_index in
-
+         
          G.snoc_unique_lemma h_index f';*)
          lemma_tl h_index f';
          let f'' = cons h_index f' in
@@ -773,7 +1560,7 @@ let rec get_allocs_helper (g:heap{Seq.length (objects2 0UL g) > 0})
                                                (G.is_vertex_set allocs) /\
                                                (forall x. Seq.mem x allocs ==> Seq.mem x f) /\
                                                (G.subset_vertices allocs f) /\
-                                               (forall x. Seq.mem x allocs ==>
+                                               (forall x. Seq.mem x allocs ==> 
                                                   Seq.mem x (objects2 0UL g)) /\
                                                (forall x. Seq.mem x allocs ==> Seq.mem x (objects2 0UL g)) /\
                                                (forall x. Seq.mem x allocs ==> (isWhiteObject1 x g) \/ (isGrayObject1 x g) \/
@@ -785,8 +1572,8 @@ let rec get_allocs_helper (g:heap{Seq.length (objects2 0UL g) > 0})
                                                (forall x. Seq.mem x f /\ (isWhiteObject1 x g) ==> Seq.mem x allocs) /\
                                                (forall x. Seq.mem x f /\ (isBlackObject1 x g) ==> Seq.mem x allocs) /\
                                                (forall x. Seq.mem x f /\ (isGrayObject1 x g) ==> Seq.mem x allocs)})
-                      (decreases length f) =
-if length f = 0 then
+                      (decreases length f) = 
+if length f = 0 then 
 (
  G.is_vertex_set_lemma1 f;
  assert (G.is_vertex_set f);
@@ -798,24 +1585,24 @@ else
  (
    let hd = Seq.head f in
    let tl = Seq.tail f in
-
+   
    assert (forall x. Seq.mem x f ==> Usize.v x >= 0 /\ Usize.v x < heap_size);
    assert (forall x. Seq.mem x tl ==> Usize.v x >= 0 /\ Usize.v x < heap_size);
    assert (G.is_vertex_set f);
-
+   
    G.is_vertex_set_lemma f;
    assert (G.is_vertex_set tl);
-
+   
    G.is_vertex_set_lemma4 f;
    assert (~(Seq.mem hd tl));
-
+   
    let allocs' = get_allocs_helper g tl in
    assert (forall x. Seq.mem x tl /\ (isWhiteObject1 x g) ==> Seq.mem x allocs');
    assert (forall x. Seq.mem x allocs' ==> Seq.mem x tl);
    assert (~(Seq.mem hd allocs'));
    assert (Seq.mem hd f);
    objects2_color_lemma 0UL g;
-   assert (forall x. Seq.mem x (objects2 0UL g) ==> color_of_object1 x g == white \/
+   assert (forall x. Seq.mem x (objects2 0UL g) ==> color_of_object1 x g == white \/ 
                                                color_of_object1 x g == gray \/
                                                color_of_object1 x g == black \/
                                                color_of_object1 x g == blue);
@@ -834,7 +1621,7 @@ else
           assert (G.is_vertex_set allocs'');
           assert (G.subset_vertices allocs'' f);
           allocs''
-
+          
        )
        else
        (
@@ -855,7 +1642,7 @@ else
          assert (G.subset_vertices allocs'' f);
          allocs''
        )
-
+       
      )
    else
      (
@@ -875,9 +1662,9 @@ let snoc_equality_lemma (f: seq Usize.t{Seq.length f > 0})
                   (requires f == f' /\ hd == hd')
                   (ensures (snoc f hd == snoc f' hd')) = ()
 
-#restart-solver
+#restart-solver 
 
-#restart-solver
+#restart-solver 
 
 #restart-solver
 
@@ -894,14 +1681,14 @@ let seq_length_tl_lemma (f: seq Usize.t{Seq.length f > 0})
 let seq_empty_length_lemma ()
             : Lemma
               (ensures (Seq.length (Seq.empty) == 0)) = ()
-
+              
 let seq_cons_length_mem_lemma (hd:Usize.t)
                    : Lemma
                      (ensures (Seq.length (Seq.cons hd (Seq.empty)) == 1) /\
                               (Seq.head (Seq.cons hd (Seq.empty)) == hd) /\
                               (Seq.tail (Seq.cons hd (Seq.empty)) == Seq.empty)) = ()
 
-let seq_empty_mem_lemma (#a:eqtype)
+let seq_empty_mem_lemma (#a:eqtype) 
             : Lemma
               (ensures ~(exists x.Seq.mem x (Seq.empty #a))) = ()
 
@@ -933,23 +1720,23 @@ let rec get_allocs_helper_lemma (g:heap{Seq.length (objects2 0UL g) > 0})
                                   (Seq.length g == Seq.length g') /\
                                   (heap_remains_same_except_index_v_id v_id g g') /\
                                   (color_of_object1 v_id g' == c) /\
-                                  (color_of_object1 v_id g == white \/ color_of_object1 v_id g == gray \/
+                                  (color_of_object1 v_id g == white \/ color_of_object1 v_id g == gray \/ 
                                     color_of_object1 v_id g == black) /\
                                   (wosize_of_object1 v_id g' == wosize_of_object1 v_id g) /\
                                   (tag_of_object1 v_id g' == tag_of_object1 v_id g) /\
                                   (Seq.mem v_id (objects2 0UL g)) /\
                                   (Seq.mem v_id (objects2 0UL g')) /\
                                   (c == 1UL \/ c == 2UL \/ c == 3UL))
-                         (ensures (get_allocs_helper g f == get_allocs_helper g' f'))
-                         (decreases (Seq.length f))=
-if length f = 0 then
+                         (ensures (get_allocs_helper g f == get_allocs_helper g' f')) 
+                         (decreases (Seq.length f))= 
+if length f = 0 then 
   (
      G.is_vertex_set_lemma1 f;
      assert (G.is_vertex_set f);
      assert (G.subset_vertices f f);
      assert (get_allocs_helper g f == get_allocs_helper g' f');
      ()
-)
+) 
 else
  (
    let hd = Seq.head f in
@@ -969,7 +1756,7 @@ else
    assert (tl == tail f);
    assert (G.is_vertex_set tl);
    assert (G.is_vertex_set tl');
-
+   
    G.is_vertex_set_lemma4 f;
    G.is_vertex_set_lemma4 f';
    seq_mem_lemma f;
@@ -981,7 +1768,7 @@ else
 
    //assert (G.is_vertex_set tl);
    assert (get_allocs_helper g tl == get_allocs_helper g' tl');
-
+  
    if (isWhiteObject1 hd g || isGrayObject1 hd g || isBlackObject1 hd g) then
      (
        assert (isWhiteObject1 hd g || isGrayObject1 hd g || isBlackObject1 hd g);
@@ -994,7 +1781,7 @@ else
           Seq.lemma_mem_snoc allocs'' hd';
           let allocs1 = snoc allocs' hd in
           let allocs2 = snoc allocs'' hd' in
-
+          
           G.snoc_unique_lemma hd allocs';
           G.snoc_unique_lemma hd' allocs'';
           assert (allocs'' == allocs');
@@ -1024,7 +1811,7 @@ else
          assert (forall x. Seq.mem x allocs1 ==> Seq.mem x f);
          assert (G.subset_vertices allocs1 f);
          ()
-
+         
        )
      )
    else
@@ -1038,13 +1825,13 @@ else
 #push-options "--split_queries always"
 
 
-let get_allocated_block_addresses   (g:heap {Seq.length (objects2 0UL g) > 0})
+let get_allocated_block_addresses   (g:heap {Seq.length (objects2 0UL g) > 0}) 
                           : Tot (allocs: seq Usize.t {(forall x. Seq.mem x allocs ==> Usize.v x >= 0 /\ Usize.v x < heap_size) /\
                                                       (forall x. Seq.mem x allocs ==> is_hp_addr x) /\
                                                       (forall x. Seq.mem x allocs ==> Seq.mem x (objects2 0UL g)) /\
                                                       (G.is_vertex_set allocs) /\
                                                       (G.subset_vertices allocs (objects2 0UL g)) /\
-                                                      (forall x. Seq.mem x allocs ==> (isWhiteObject1 x g) \/
+                                                      (forall x. Seq.mem x allocs ==> (isWhiteObject1 x g) \/ 
                                                                                  (isGrayObject1 x g) \/
                                                                                 (isBlackObject1 x g)) /\
                                                       (forall x. Seq.mem x (objects2 0UL g) /\
@@ -1055,7 +1842,7 @@ let f =  objects2 0UL g in
    assert (forall x. Seq.mem x f ==> Usize.v x >= 0 /\ Usize.v x < heap_size);
    assert (G.is_vertex_set f);
    assert (forall x. Seq.mem x f ==> Usize.v x >= 0);
-
+   
    let allocs = get_allocs_helper g f in
    assert (G.is_vertex_set allocs);
    assert (G.subset_vertices allocs f);
@@ -1082,7 +1869,7 @@ let cons_lemma_mem (hd:Usize.t)
  Seq.mem_cons hd l;
  ()
 
-#restart-solver
+#restart-solver 
 
 #restart-solver
 
@@ -1097,21 +1884,21 @@ let cons_lemma_mem (hd:Usize.t)
 let rec is_fields_contents_within_limit2_lemma_for_sweep   (h_index: hp_addr)
                                                            (wz: wosize{is_fields_within_limit1 h_index wz})
                                                            (wz': wosize{is_fields_within_limit1 h_index wz'})
-                                                           (g:heap{Seq.length (objects2 0UL g) > 0})
+                                                           (g:heap{Seq.length (objects2 0UL g) > 0}) 
                                                            (g':heap{Seq.length (objects2 0UL g') > 0})
-
+                                          
                           : Lemma
                             (requires (wz == wz') /\
                                       (Seq.mem h_index (get_allocated_block_addresses g) /\
                                        Seq.mem h_index (get_allocated_block_addresses g')) /\
                                       (forall y.   Usize.v y >= Usize.v h_index + Usize.v mword /\
-                                                   Usize.v y <=
+                                                   Usize.v y <= 
                                                      Usize.v h_index + (Usize.v wz * Usize.v mword) ==>
                                                                      read_word g y == read_word g' y) /\
-                                      is_fields_contents_within_limit2 h_index wz g == true
-
+                                      is_fields_contents_within_limit2 h_index wz g == true 
+                                      
                             )
-
+                                                                 
                             (ensures (*(is_fields_contents_within_limit2 h_index wz g == true <==>*)
                                       is_fields_contents_within_limit2 h_index wz' g' == true)
                             (decreases (Usize.v wz)) =
@@ -1132,10 +1919,10 @@ let rec is_fields_contents_within_limit2_lemma_for_sweep   (h_index: hp_addr)
     assert (succ == succ');
     if (isPointer s g) then
    (
-
+     
      if Usize.v succ >= Usize.v mword && Usize.v succ < heap_size && is_hp_addr succ then
          is_fields_contents_within_limit2_lemma_for_sweep h_index wz1 wz2 g g'
-
+        
      else
          ()
    )
@@ -1153,12 +1940,12 @@ let rec get_color_based_block_picker (g:heap{Seq.length (objects2 0UL g) > 0})
                                                       (G.is_vertex_set f) /\
                                                       (G.subset_vertices f (objects2 0UL g)) /\
                                                       (forall x. Seq.mem x f ==> Seq.mem x (objects2 0UL g)) /\
-                                                      (forall x. Seq.mem x f ==> (isWhiteObject1 x g) \/
+                                                      (forall x. Seq.mem x f ==> (isWhiteObject1 x g) \/ 
                                                                             (isGrayObject1 x g) \/
                                                                             (isBlackObject1 x g))})
-
+                                                               
                                      (c:color{c == white \/ c == gray \/ c == black})
-
+                                     
                     : Tot (color_block: seq Usize.t{(forall x. Seq.mem x color_block ==> Usize.v x >= 0 /\ Usize.v x < heap_size)  /\
                                                     (forall x. Seq.mem x color_block ==> Usize.v x % Usize.v mword == 0) /\
                                                     (G.is_vertex_set color_block) /\
@@ -1169,12 +1956,12 @@ let rec get_color_based_block_picker (g:heap{Seq.length (objects2 0UL g) > 0})
                                                     (forall x. Seq.mem x color_block ==> Seq.mem x f /\ color_of_object1 x g == c) /\
                                                     (forall x. Seq.mem x f /\ color_of_object1 x g == c ==> Seq.mem x color_block) /\
                                                     (forall x. Seq.mem x color_block <==> Seq.mem x f /\ color_of_object1 x g == c)})
-
+                                            
                       (decreases length f) =
-assert (forall x. Seq.mem x f ==>  color_of_object1 x g == black \/
-                             color_of_object1 x g == white \/
-                             color_of_object1 x g == gray);
-if length f = 0 then
+assert (forall x. Seq.mem x f ==>  color_of_object1 x g == black \/ 
+                             color_of_object1 x g == white \/ 
+                             color_of_object1 x g == gray);                   
+if length f = 0 then 
 (
  G.is_vertex_set_lemma1 f;
  assert (G.is_vertex_set f);
@@ -1188,11 +1975,11 @@ else
  (
     let hd = Seq.head f in
     let tl = Seq.tail f in
-
+   
     G.is_vertex_set_lemma f;
-
+    
     G.is_vertex_set_lemma4 f;
-
+    
     let color_block' = get_color_based_block_picker g tl c in
     assert (forall x. Seq.mem x color_block' ==> Seq.mem x tl);
     assert (~(Seq.mem hd color_block'));
@@ -1214,7 +2001,7 @@ else
           )
         else
           (
-             Seq.lemma_tl hd color_block';
+             Seq.lemma_tl hd color_block'; 
              let color_block'' = Seq.cons hd color_block' in
              assert (~(Seq.mem hd color_block'));
              G.is_vertex_set_cons hd color_block';
@@ -1230,7 +2017,7 @@ else
              color_block''
           )
      )
-
+    
     else
      (
         assert (G.is_vertex_set color_block');
@@ -1246,100 +2033,96 @@ else
 
 #restart-solver
 
-let get_allocated_block_addresses_lemma g g' v_id c =
+let get_allocated_block_addresses_lemma g g' v_id c = 
   let f =  objects2 0UL g in
   let f' = objects2 0UL g' in
   assert (f == f');
   let allocs1 = get_allocs_helper g f in
   let allocs2 = get_allocs_helper g' f' in
-  get_allocs_helper_lemma g g' f f' v_id c;
+  get_allocs_helper_lemma g g' f f' v_id c; 
   assert (allocs1 == allocs2);
   assert (get_allocated_block_addresses g == get_allocated_block_addresses g');
   ()
 
 #reset-options "--z3rlimit 500"
 
-let get_black_block_addresses g f =
+let get_black_block_addresses g f = 
  let blacks =  get_color_based_block_picker g f black in
  assert (Seq.equal f (get_allocated_block_addresses g));
  assert ((forall x. Seq.mem x f ==> (isWhiteObject1 x g) \/ (isGrayObject1 x g) \/ (isBlackObject1 x g)) /\
-         (forall x. Seq.mem x (objects2 0UL g) /\
+         (forall x. Seq.mem x (objects2 0UL g) /\ 
                                ((isWhiteObject1 x g) \/ (isGrayObject1 x g) \/ (isBlackObject1 x g))==>
                                                       Seq.mem x f));
  assert (forall x. Seq.mem x f /\ color_of_object1 x g == black ==> Seq.mem x blacks);
  assert (forall x. Seq.mem x (objects2 0UL g) /\ isBlackObject1 x g ==>
                                                       Seq.mem x blacks);
  assert (forall x. Seq.mem x blacks ==> Seq.mem x (objects2 0UL g) /\ isBlackObject1 x g);
- assert (forall x. Seq.mem x blacks <==> Seq.mem x (objects2 0UL g) /\ isBlackObject1 x g);
+ assert (forall x. Seq.mem x blacks <==> Seq.mem x (objects2 0UL g) /\ isBlackObject1 x g);                                             
  assert (forall x. Seq.mem x blacks ==> Usize.v x >= 0 /\ Usize.v x < heap_size);
  assert (G.is_vertex_set blacks);
  assert (forall x. Seq.mem x blacks ==> Seq.mem x f);
  assert (G.subset_vertices blacks f /\
         (G.subset_vertices blacks (objects2 0UL g)));
  assert (forall x. Seq.mem x blacks ==> color_of_object1 x g == black);
- assert (forall x. Seq.mem x blacks <==> Seq.mem x f /\ color_of_object1 x g == black);
+ assert (forall x. Seq.mem x blacks <==> Seq.mem x f /\ color_of_object1 x g == black); 
  assert (Seq.equal f (get_allocated_block_addresses g));
- assert (forall x. Seq.mem x blacks <==> Seq.mem x (get_allocated_block_addresses g) /\ color_of_object1 x g == black);
+ assert (forall x. Seq.mem x blacks <==> Seq.mem x (get_allocated_block_addresses g) /\ color_of_object1 x g == black); 
  blacks
 
-#restart-solver
+#restart-solver 
 
 
-let get_gray_block_addresses g f =
+let get_gray_block_addresses g f = 
  let grays =  get_color_based_block_picker g f 2UL in
  assert (Seq.equal f (get_allocated_block_addresses g));
  assert ((forall x. Seq.mem x f ==> (isWhiteObject1 x g) \/ (isGrayObject1 x g) \/ (isBlackObject1 x g)) /\
-         (forall x. Seq.mem x (objects2 0UL g) /\
+         (forall x. Seq.mem x (objects2 0UL g) /\ 
                                ((isWhiteObject1 x g) \/ (isGrayObject1 x g) \/ (isBlackObject1 x g))==>
                                                       Seq.mem x f));
  assert (forall x. Seq.mem x f /\ color_of_object1 x g == gray ==> Seq.mem x grays);
  assert (forall x. Seq.mem x (objects2 0UL g) /\ isGrayObject1 x g ==>
                                                       Seq.mem x grays);
  assert (forall x. Seq.mem x grays ==> Seq.mem x (objects2 0UL g) /\ isGrayObject1 x g);
- assert (forall x. Seq.mem x grays <==>
-   Seq.mem x (objects2 0UL g) /\ isGrayObject1 x g);
+ assert (forall x. Seq.mem x grays <==> 
+   Seq.mem x (objects2 0UL g) /\ isGrayObject1 x g);                                             
  assert (forall x. Seq.mem x grays ==> Usize.v x >= 0 /\ Usize.v x < heap_size);
  assert (G.is_vertex_set grays);
  assert (forall x. Seq.mem x grays ==> Seq.mem x f);
  assert (G.subset_vertices grays f /\
           (G.subset_vertices  grays (objects2 0UL g)));
  assert (forall x. Seq.mem x grays ==> color_of_object1 x g == gray);
- assert (forall x. Seq.mem x grays <==> Seq.mem x f /\ color_of_object1 x g == gray);
+ assert (forall x. Seq.mem x grays <==> Seq.mem x f /\ color_of_object1 x g == gray); 
  assert (Seq.equal f (get_allocated_block_addresses g));
- assert (forall x. Seq.mem x grays <==> Seq.mem x (get_allocated_block_addresses g) /\ color_of_object1 x g == gray);
+ assert (forall x. Seq.mem x grays <==> Seq.mem x (get_allocated_block_addresses g) /\ color_of_object1 x g == gray); 
  grays
 
-#restart-solver
+#restart-solver 
 
-let get_white_block_addresses g f =
+let get_white_block_addresses g f = 
  let whites =  get_color_based_block_picker g f white in
  assert (Seq.equal f (get_allocated_block_addresses g));
  assert ((forall x. Seq.mem x f ==> (isWhiteObject1 x g) \/ (isGrayObject1 x g) \/ (isBlackObject1 x g)) /\
-         (forall x. Seq.mem x (objects2 0UL g) /\
+         (forall x. Seq.mem x (objects2 0UL g) /\ 
                                ((isWhiteObject1 x g) \/ (isGrayObject1 x g) \/ (isBlackObject1 x g))==>
                                                       Seq.mem x f));
  assert (forall x. Seq.mem x f /\ color_of_object1 x g == white ==> Seq.mem x whites);
  assert (forall x. Seq.mem x (objects2 0UL g) /\ isWhiteObject1 x g ==>
                                                       Seq.mem x whites);
  assert (forall x. Seq.mem x whites ==> Seq.mem x (objects2 0UL g) /\ isWhiteObject1 x g);
- assert (forall x. Seq.mem x whites <==>
-   Seq.mem x (objects2 0UL g) /\ isWhiteObject1 x g);
+ assert (forall x. Seq.mem x whites <==> 
+   Seq.mem x (objects2 0UL g) /\ isWhiteObject1 x g);                                             
  assert (forall x. Seq.mem x whites ==> Usize.v x >= 0 /\ Usize.v x < heap_size);
  assert (G.is_vertex_set whites);
  assert (forall x. Seq.mem x whites ==> Seq.mem x f);
  assert (G.subset_vertices whites f /\
           (G.subset_vertices whites (objects2 0UL g)));
  assert (forall x. Seq.mem x whites ==> color_of_object1 x g == white);
- assert (forall x. Seq.mem x whites <==> Seq.mem x f /\ color_of_object1 x g == white);
+ assert (forall x. Seq.mem x whites <==> Seq.mem x f /\ color_of_object1 x g == white); 
  assert (Seq.equal f (get_allocated_block_addresses g));
- assert (forall x. Seq.mem x whites <==> Seq.mem x (get_allocated_block_addresses g) /\ color_of_object1 x g == white);
+ assert (forall x. Seq.mem x whites <==> Seq.mem x (get_allocated_block_addresses g) /\ color_of_object1 x g == white); 
  whites
 
-#restart-solver
-
-#reset-options "--split_queries always"
-
-let rec is_fields_contents_within_limit2_lemma  h_index wz wz' g g' =
+let rec is_fields_contents_within_limit2_lemma  h_index wz wz' g g' = 
   if (Usize.v wz = 0) then ()
  else
  (
@@ -1369,8 +2152,8 @@ let rec is_fields_contents_within_limit2_lemma  h_index wz wz' g g' =
       ()
    )
  )
-
-let rec check_all_block_fields_within_limit2 g f' =
+                            
+let rec check_all_block_fields_within_limit2 g f' = 
   match length f' with
    | 0 -> true
    | _ -> assert (length f' > 0);
@@ -1379,12 +2162,12 @@ let rec check_all_block_fields_within_limit2 g f' =
          assert (Usize.v hd % Usize.v mword == 0);
          let wz = getWosize (read_word g hd) in
          if (is_fields_contents_within_limit2 hd wz g) then
-            (
+            (  
                assert (is_fields_contents_within_limit2 hd wz g);
                check_all_block_fields_within_limit2 g tl
             )
             else
-             false
+             false 
 
 
 
@@ -1394,7 +2177,7 @@ let rec check_all_block_fields_within_limit2 g f' =
 
 #push-options "--split_queries always"
 
-#restart-solver
+#restart-solver 
 
 let rec check_all_block_fields_within_limit2_lemma g g' f' f'' =
  match length f' with
@@ -1402,12 +2185,12 @@ let rec check_all_block_fields_within_limit2_lemma g g' f' f'' =
    | _ -> assert (length f' > 0);
          let hd = Seq.head f' in
          let hd' = Seq.head f'' in
-
-
+         
+         
          let tl = Seq.tail f' in
          let tl' = Seq.tail f'' in
 
-
+        
 
          let wz = getWosize (read_word g hd) in
          let wz' = getWosize (read_word g' hd') in
@@ -1417,45 +2200,45 @@ let rec check_all_block_fields_within_limit2_lemma g g' f' f'' =
 
          assert (wz == wz');
 
-         assert (forall (i:Usize.t {Usize.v i > 0 /\ Usize.v i <= Usize.v wz}). Usize.v (Usize.add hd (Usize.mul i mword)) < heap_size);
+         assert (forall (i:Usize.t {Usize.v i > 0 /\ Usize.v i <= Usize.v wz}). Usize.v (Usize.add hd (Usize.mul i mword)) < heap_size); 
 
          h_index_field_index_all_mword_multiple_lemma1 g hd;
          assert (forall (i:Usize.t {Usize.v i > 0 /\ Usize.v i <= Usize.v wz}). Usize.v (Usize.add hd (Usize.mul i mword)) % Usize.v mword == 0);
-         assert (forall (i:Usize.t {Usize.v i > 0 /\ Usize.v i <= Usize.v wz}).
+         assert (forall (i:Usize.t {Usize.v i > 0 /\ Usize.v i <= Usize.v wz}). 
                                                     (*(is_hp_addr ((Usize.add h_index (Usize.mul i mword)))) /\ (*Mandatory condition, since z3 is not detecting modular
                                                                                                                arithmetic conditions*)
                                                     isPointer (Usize.add h_index (Usize.mul i mword)) g ==>*)
-                                                    Usize.v (read_word g (Usize.add hd (Usize.mul i mword))) ==
+                                                    Usize.v (read_word g (Usize.add hd (Usize.mul i mword))) == 
                                                     Usize.v (read_word g' (Usize.add hd (Usize.mul i mword))));
-
+                                             
          is_fields_contents_within_limit2_lemma hd wz wz' g g';
-
+         
          if (is_fields_contents_within_limit2 hd wz g) then
-            (
-
+            (  
+              
                check_all_block_fields_within_limit2_lemma g g' tl tl';
                ()
             )
          else
            ()
-
+         
 
 
 
 #reset-options "--z3rlimit 50 --max_fuel 0 --max_ifuel 0 --using_facts_from '* -FStar.Seq'"
 
-#restart-solver
+#restart-solver 
 
-let rec is_fields_points_to_blocks2_test      (h_index: hp_addr)
+let rec is_fields_points_to_blocks2_test      (h_index: hp_addr) 
                                           (g:heap{Seq.length (objects2 0UL g) > 0})
                                           (wz: wosize{(is_fields_within_limit1 h_index wz /\
-                                               is_fields_contents_within_limit2 h_index wz g)})
+                                               is_fields_contents_within_limit2 h_index wz g)}) 
                                           (f':seq Usize.t { (forall x. Seq.mem x f' ==> is_hp_addr x) /\
-                                                    (forall x. Seq.mem x f' ==>
+                                                    (forall x. Seq.mem x f' ==> 
                                                      Seq.mem x (get_allocated_block_addresses g))})
-
+                                 
                    : Tot (b:bool{b == true <==> is_fields_points_to_blocks2_post_condition h_index g wz f'})
-                    (decreases (Usize.v wz)) =
+                    (decreases (Usize.v wz)) = 
  assert (is_hp_addr h_index);
  if (Usize.v wz = 0) then true
   else
@@ -1473,7 +2256,7 @@ let rec is_fields_points_to_blocks2_test      (h_index: hp_addr)
     assert (is_hp_addr s);
     if (isPointer s g) then
     (
-
+      
       lemma_len_slice g (Usize.v s) ((Usize.v s) + (Usize.v mword));
       let succ = read_word g s in
       assert (Usize.v succ >= Usize.v mword);
@@ -1492,7 +2275,7 @@ let rec is_fields_points_to_blocks2_test      (h_index: hp_addr)
         )
         else
         (
-          false
+          false 
         )
       )
       else
@@ -1518,15 +2301,15 @@ let rec is_fields_points_to_blocks2_test      (h_index: hp_addr)
           )
           else
           (
-            false
+            false 
           )
         )
         else
         (
-          false
+          false 
         )
       )
-
+     
     )
     else
     (
@@ -1534,11 +2317,11 @@ let rec is_fields_points_to_blocks2_test      (h_index: hp_addr)
       let b = is_fields_points_to_blocks2_test h_index g wz' f' in
       b
     )
-
+ 
   )
 
 
-let rec is_fields_points_to_blocks2 h_index g wz f' =
+let rec is_fields_points_to_blocks2 h_index g wz f' = 
 assert (is_hp_addr h_index);
  if (Usize.v wz = 0) then true
   else
@@ -1556,7 +2339,7 @@ assert (is_hp_addr h_index);
     assert (is_hp_addr s);
     if (isPointer s g) then
     (
-
+      
       lemma_len_slice g (Usize.v s) ((Usize.v s) + (Usize.v mword));
       let succ = read_word g s in
       assert (Usize.v succ >= Usize.v mword);
@@ -1575,7 +2358,7 @@ assert (is_hp_addr h_index);
         )
         else
         (
-          false
+          false 
         )
       )
       else
@@ -1601,15 +2384,15 @@ assert (is_hp_addr h_index);
           )
           else
           (
-            false
+            false 
           )
         )
         else
         (
-          false
+          false 
         )
       )
-
+     
     )
     else
     (
@@ -1617,11 +2400,11 @@ assert (is_hp_addr h_index);
       let b = is_fields_points_to_blocks2_test h_index g wz' f' in
       b
     )
-
+ 
   )
 
 
-#restart-solver
+#restart-solver 
 
 #restart-solver
 
@@ -1631,16 +2414,16 @@ assert (is_hp_addr h_index);
 
 #restart-solver
 
-let rec is_fields_points_to_blocks2_lemma1  (h_index: hp_addr)
-                                        (g:heap{Seq.length (objects2 0UL g) > 0})
+let rec is_fields_points_to_blocks2_lemma1  (h_index: hp_addr) 
+                                        (g:heap{Seq.length (objects2 0UL g) > 0}) 
                                         (wz: wosize{(is_fields_within_limit1 h_index wz /\
-                                                     is_fields_contents_within_limit2 h_index wz g)})
+                                                     is_fields_contents_within_limit2 h_index wz g)}) 
                                         (f':seq Usize.t { (forall x. Seq.mem x f' ==> Usize.v x >= 0 /\ Usize.v x < heap_size) /\
                                                           (forall x. Seq.mem x f' ==> is_hp_addr x) /\
                                                           (forall x. Seq.mem x f' ==> Seq.mem x (get_allocated_block_addresses g))})
-                                        (g':heap{Seq.length (objects2 0UL g') > 0})
+                                        (g':heap{Seq.length (objects2 0UL g') > 0}) 
                                         (wz1: wosize{(is_fields_within_limit1 h_index wz1 /\
-                                                      is_fields_contents_within_limit2 h_index wz1 g')})
+                                                      is_fields_contents_within_limit2 h_index wz1 g')}) 
                                         (f'':seq Usize.t { (forall x. Seq.mem x f'' ==> Usize.v x >= 0 /\ Usize.v x < heap_size) /\
                                                            (forall x. Seq.mem x f'' ==> is_hp_addr x) /\
                                                            (forall x. Seq.mem x f'' ==> Seq.mem x (get_allocated_block_addresses g'))})
@@ -1650,11 +2433,11 @@ let rec is_fields_points_to_blocks2_lemma1  (h_index: hp_addr)
                                             (objects2 0UL g == objects2 0UL g') /\
                                             (get_allocated_block_addresses g == get_allocated_block_addresses g') (*/\
                                       (forall x. Usize.v x  >= Usize.v h_index + Usize.v mword /\
-                                            Usize.v x <= Usize.v h_index + (Usize.v wz * Usize.v mword) ==>
+                                            Usize.v x <= Usize.v h_index + (Usize.v wz * Usize.v mword) ==> 
                                             (length (slice g' (Usize.v x) ((Usize.v x) + (Usize.v mword))) = 8)) /\
-
+                                      
                                       (forall x. Usize.v x  >= Usize.v h_index + Usize.v mword /\
-                                            Usize.v x <= Usize.v h_index + (Usize.v wz * Usize.v mword) ==>
+                                            Usize.v x <= Usize.v h_index + (Usize.v wz * Usize.v mword) ==> 
                                             (length (slice g (Usize.v x) ((Usize.v x) + (Usize.v mword))) = 8))*) /\
 
                                       (forall (x:Usize.t{Usize.v x < heap_size /\ Usize.v x % 8 == 0}). wosize_of_object1 x g ==
@@ -1666,7 +2449,7 @@ let rec is_fields_points_to_blocks2_lemma1  (h_index: hp_addr)
                                             Usize.v x <= Usize.v h_index + (Usize.v wz * Usize.v mword) ==> read_word g x == read_word g' x))
                                   (ensures is_fields_points_to_blocks2 h_index g wz f' == true <==>
                                             is_fields_points_to_blocks2 h_index g' wz1 f'' == true)
-                                  (decreases (Usize.v wz)) =
+                                  (decreases (Usize.v wz)) = 
  if (Usize.v wz = 0) then ()
   else
   (
@@ -1691,12 +2474,12 @@ let rec is_fields_points_to_blocks2_lemma1  (h_index: hp_addr)
       let succ = read_word g s in
       let succ' = read_word g' s in
       assert (succ == succ');
-
+      
       assert (Usize.v succ >= Usize.v mword);
       assert (Usize.v succ < heap_size);
       assert (Usize.v succ % Usize.v mword == 0);
       assert (is_hp_addr succ);
-
+      
       let hdr_succ = hd_address succ in
       let hdr_succ1 = hd_address succ' in
       assert (hdr_succ = hdr_succ1);
@@ -1716,14 +2499,14 @@ let rec is_fields_points_to_blocks2_lemma1  (h_index: hp_addr)
           assert (is_fields_points_to_blocks2 h_index g wz' f' == true <==>
                                             is_fields_points_to_blocks2 h_index g' wz2 f'' == true);
           ()
-
+  
         )
         else
         (
           ()
         )
       )
-
+      
       else
       (
         assert (Usize.v tg == infix_tag);
@@ -1772,18 +2555,18 @@ let rec is_fields_points_to_blocks2_lemma1  (h_index: hp_addr)
     else
     (
        assert (~(isPointer s g));
-
+     
        is_fields_points_to_blocks2_lemma1 h_index g wz' f' g' wz2 f'';
        ()
     )
   )
 
-#restart-solver
+#restart-solver 
 
-#restart-solver
+#restart-solver 
 
 
-let rec is_fields_points_to_blocks2_lemma h_index g wz f' g' wz1 f'' =
+let rec is_fields_points_to_blocks2_lemma h_index g wz f' g' wz1 f'' = 
   if (Usize.v wz = 0) then ()
   else
   (
@@ -1808,12 +2591,12 @@ let rec is_fields_points_to_blocks2_lemma h_index g wz f' g' wz1 f'' =
       let succ = read_word g s in
       let succ' = read_word g' s in
       assert (succ == succ');
-
+      
       assert (Usize.v succ >= Usize.v mword);
       assert (Usize.v succ < heap_size);
       assert (Usize.v succ % Usize.v mword == 0);
       assert (is_hp_addr succ);
-
+      
       let hdr_succ = hd_address succ in
       let hdr_succ1 = hd_address succ' in
       assert (hdr_succ = hdr_succ1);
@@ -1833,14 +2616,14 @@ let rec is_fields_points_to_blocks2_lemma h_index g wz f' g' wz1 f'' =
           assert (is_fields_points_to_blocks2 h_index g wz' f' == true <==>
                                             is_fields_points_to_blocks2 h_index g' wz2 f'' == true);
           ()
-
+  
         )
         else
         (
           ()
         )
       )
-
+      
       else
       (
         assert (Usize.v tg == infix_tag);
@@ -1889,7 +2672,7 @@ let rec is_fields_points_to_blocks2_lemma h_index g wz f' g' wz1 f'' =
     else
     (
        assert (~(isPointer s g));
-
+     
        is_fields_points_to_blocks2_lemma h_index g wz' f' g' wz2 f'';
        ()
     )
@@ -1898,15 +2681,15 @@ let rec is_fields_points_to_blocks2_lemma h_index g wz f' g' wz1 f'' =
 
 #restart-solver
 
-let get_allocated_block_addresses_color_lemma (g:heap {Seq.length (objects2 0UL g) > 0})
+let get_allocated_block_addresses_color_lemma (g:heap {Seq.length (objects2 0UL g) > 0}) 
                                               (x:hp_addr{Seq.mem x (objects2 0UL g)})
                 : Lemma
                   (requires color_of_object1 x g == white)
-                  (ensures (Seq.mem x (get_allocated_block_addresses g))) =
+                  (ensures (Seq.mem x (get_allocated_block_addresses g))) = 
   assert (forall x. Seq.mem x (objects2 0UL g) /\
                     ((isWhiteObject1 x g) \/ (isGrayObject1 x g) \/ (isBlackObject1 x g))==>
                      Seq.mem x (get_allocated_block_addresses g));
-
+  
   assert (Seq.mem x (get_allocated_block_addresses g));
   ()
 
@@ -1914,175 +2697,223 @@ let get_allocated_block_addresses_color_lemma (g:heap {Seq.length (objects2 0UL 
 
 (*assume (Usize.v f_index_new >= heap_size ==> ~(Seq.mem h_index_new (objects2 h_index g)));*)
 
+#restart-solver
 
 
-(*let rec is_fields_points_to_blocks2_lemma_for_sweep  (h_index: hp_addr)
-                                                     (g:heap{Seq.length (objects2 0UL g) > 0})
-                                                     (wz: wosize{(is_fields_within_limit1 h_index wz /\
-                                                                  is_fields_contents_within_limit2 h_index wz g)})
-                                                     (f':seq Usize.t { (forall x. Seq.mem x f' ==>
-                                                                        Usize.v x >= 0 /\ Usize.v x < heap_size) /\
-                                                                        (forall x. Seq.mem x f' ==> is_hp_addr x) /\
-                                                                        (forall x. Seq.mem x f' ==>
-                                                                               Seq.mem x (get_allocated_block_addresses g)) /\
-                                                                        (forall x. Seq.mem x f' ==>
-                                                                                is_fields_within_limit1 x (getWosize (read_word g x)))})
+let check_well_formed_closure_objs_lemma1_pre1  (g:heap{Seq.length (objects2 0UL g) > 0})
+                                               (g':heap{Seq.length (objects2 0UL g') > 0})
+                                          
+                                               (f':seq Usize.t {(forall x. Seq.mem x f' ==> Usize.v x >= 0 /\ Usize.v x < heap_size) /\
+                                                                  (forall x. Seq.mem x f' ==> Usize.v x % Usize.v mword == 0) /\
+                                                                  (forall x. Seq.mem x f' ==> Seq.mem x (get_allocated_block_addresses g')) /\
+                                                                   
+                                                                  (forall x. Seq.mem x f' ==> is_fields_within_limit1 x (getWosize (read_word g' x)))})=
+      (forall x y. Seq.mem x f' /\ 
+                   Usize.v y >= Usize.v x + Usize.v mword /\
+                   Usize.v y <= Usize.v x + (Usize.v (getWosize (read_word g x)) * Usize.v mword) ==>
+                                                                     read_word g y == read_word g' y)
 
-                                                     (g':heap{Seq.length (objects2 0UL g') > 0})
-                                                     (wz1: wosize{(is_fields_within_limit1 h_index wz1 /\
-                                                                   is_fields_contents_within_limit2 h_index wz1 g')})
-                                                     (f'':seq Usize.t { (forall x. Seq.mem x f'' ==>
-                                                                          Usize.v x >= 0 /\ Usize.v x < heap_size) /\
-                                                                        (forall x. Seq.mem x f'' ==> is_hp_addr x) /\
-                                                                        (forall x. Seq.mem x f'' ==>
-                                                                                   Seq.mem x (get_allocated_block_addresses g')) /\
-                                                                       (forall x. Seq.mem x f'' ==>
-                                                                            is_fields_within_limit1 x (getWosize (read_word g' x)))})
-                               : Lemma
-                                  (requires (wz == wz1) /\
-                                            (wz == getWosize (read_word g h_index)) /\
-                                            (wz1 == getWosize (read_word g' h_index)) /\
-                                            (Seq.mem h_index f'') /\
-                                            (forall x. Seq.mem x f'' ==> Seq.mem x f')  /\
-                                            (*(objects2 0UL g == objects2 0UL g') /\*)
-                                            (forall x. Seq.mem x (get_allocated_block_addresses g') ==>
-                                                       Seq.mem x (get_allocated_block_addresses g))  /\
-                                            (forall x. Seq.mem x (get_allocated_block_addresses g') ==>
-                                               getWosize (read_word g x) ==
-                                               getWosize (read_word g' x)) /\
-                                            (forall x. Seq.mem x (get_allocated_block_addresses g') ==>
-                                               getTag (read_word g x) ==
-                                               getTag (read_word g' x)) /\
-                                        check_well_formed_closure_objs_lemma1_pre g g' f'' /\
-                                        is_fields_points_to_blocks2 h_index g wz f'
-                                      )
-                                  (ensures is_fields_points_to_blocks2 h_index g' wz1 f'' == true
-                                            )
-                                  (decreases (Usize.v wz)) =
-  (*if (Usize.v wz = 0) then ()
-  else
-  (
-    assert (Usize.v wz > 0);
-    //get the successor_index = h_index + wz * mword
-    let s = Usize.add h_index (Usize.mul wz mword) in
+(*Suppose, fields points to block2 property is true in the heap before g2.
+  That is, all actual field pointers of all allocated objects points to allocated objects only.
+  Why actual field pointers term is used? Because in the case of infix fields, there is a one level in direction to take
+  the closure objects, which are the actual field pointer.
+  
+  Suppose, we have a property that, after the sweep, the following holds:
+   1. All actual field pointers of allocated objects are white
+   2. All allocated objects and only the allocated objects are white in color
+   
+   Then, during the below lemma, when we the control flow reaches each field type condition,
+     we will get that, they are white (pre-condition 1) and from precondition 2, we can prove that,
+     they are members of allocated objects. Then, recursive steps ensure the same for all.
+     Once this lemma is complete, this lemma proves the base condition for one allocated object and the recursive step
+     proves the same for all allocated objects. This completes the proof. *)
 
-    // For recursing, find wz' = wz - 1
-    let wz' = Usize.sub wz 1UL in
-    let wz2 = Usize.sub wz1 1UL in
+  (*As a first step, write the prop that states that all actual field pointers of an allocated object is white*)
 
-    wosize_times_mword_multiple_of_mword wz;
-    assert (Usize.v (Usize.mul wz mword) % Usize.v mword == 0);
+#restart-solver
 
-    sum_of_multiple_of_mword_is_multiple_of_mword h_index (Usize.mul wz mword);
-    assert ((Usize.v h_index + (Usize.v wz * Usize.v mword)) % Usize.v mword == 0);
-    assert (Usize.v s % Usize.v mword == 0);
-    assert (Usize.v s < heap_size);
-    assert (is_hp_addr s);
-    assert (check_well_formed_closure_objs_lemma1_pre g g' f'' );
-     if (isPointer s g) then
-    (
-      let succ = read_word g s in
-      let succ' = read_word g' s in
-      assert (succ == succ');
+#reset-options "--z3rlimit 500"
+#restart-solver
 
-      assert (Usize.v succ >= Usize.v mword);
-      assert (Usize.v succ < heap_size);
-      assert (Usize.v succ % Usize.v mword == 0);
-      assert (is_hp_addr succ);
+#restart-solver
 
-      let hdr_succ = hd_address succ in
-      let hdr_succ1 = hd_address succ' in
-      assert (hdr_succ = hdr_succ1);
-      let tg = tag_of_object1 hdr_succ g in
-      let tg1 = tag_of_object1 hdr_succ1 g' in
-      assume (color_of_object1 hdr_succ1 g' == white);
-      assert (Seq.mem hdr_succ1 (objects2 0UL g));
-      //assert (Seq.mem hdr_succ1 (get_allocated_block_addresses g'));
-      //assert (tg == tg1);
-      (*if (Usize.v tg <> infix_tag) then
-      (
-        assert (Usize.v tg <> infix_tag);
-        assert (get_allocated_block_addresses g == get_allocated_block_addresses g');
-        if (Seq.mem hdr_succ (get_allocated_block_addresses g)) then
-        (
-          is_fields_points_to_blocks2_lemma h_index g wz' f' g' wz2 f'';
-          assert (is_fields_points_to_blocks2 h_index g wz' f' == true <==>
-                                            is_fields_points_to_blocks2 h_index g' wz2 f'' == true);
-          ()
+#restart-solver
 
-        )
-        else
-        (
-          ()
-        )
-      )
+#restart-solver
 
-      else
-      (
-        assert (Usize.v tg == infix_tag);
-        let wz_succ = wosize_of_object1 hdr_succ g in
-        let wz_succ1 = wosize_of_object1 hdr_succ1 g' in
-        let wz_succ_offset = Usize.mul wz_succ mword in
-        let wz_succ_offset1 = Usize.mul wz_succ1 mword in
-        assert (forall (x:Usize.t{Usize.v x < heap_size /\ Usize.v x % 8 == 0}). wosize_of_object1 x g ==
-                                               wosize_of_object1 x g');
-        assert (wz_succ == wz_succ1);
-        if (UInt.fits (Usize.v succ - Usize.v wz_succ_offset) Usize.n) then
-        (
-          let actual_succ = Usize.sub succ wz_succ_offset in
-          let actual_succ1 = Usize.sub succ' wz_succ_offset1 in
-          if (Usize.v actual_succ >= Usize.v mword && is_hp_addr actual_succ) then
-          (
-             let hdr_actual_succ = hd_address actual_succ in
-             let hdr_actual_succ1 = hd_address actual_succ1 in
-             let tg_actual = tag_of_object1 hdr_actual_succ g in
-             let tg_actual1 = tag_of_object1 hdr_actual_succ1 g' in
-             assert (Usize.v hdr_actual_succ < heap_size /\ Usize.v hdr_actual_succ % 8 == 0);
-             assert (forall (x:Usize.t{Usize.v x < heap_size /\ Usize.v x % 8 == 0}). tag_of_object1 x g ==
-                                               tag_of_object1 x g');
-             assert (tg_actual == tg_actual1);
-            if (Usize.v tg_actual = closure_tag && Seq.mem hdr_actual_succ (get_allocated_block_addresses g)) then
-            (
-               is_fields_points_to_blocks2_lemma h_index g wz' f' g' wz2 f'';
-               ()
-            )
-            else
-            (
-              (*()*)
-              admit()
-            )
-          )
-          else
-          (
-            (*()*)
-            admit()
-          )
-        )
-        else
-        (
-          (*()*)
-          admit()
-        )
-      )*)
-      admit()
-    )
-    else
-    (
-       (*assert (~(isPointer s g));
+let field_reads_equal1 (g:heap{Seq.length (objects2 0UL g) > 0}) 
+                       (g':heap{Seq.length (objects2 0UL g') > 0}) =
+  
+  (forall x y. Seq.mem x (get_allocated_block_addresses g') /\ 
+                Usize.v y >= Usize.v x + Usize.v mword /\
+                Usize.v y <= Usize.v x + (Usize.v (getWosize (read_word g x)) * Usize.v mword) ==>
+                                                                     read_word g y == read_word g' y)
 
-       is_fields_points_to_blocks2_lemma h_index g wz' f' g' wz2 f'';
-       ()*)
-       admit()
-    )
-  )
-*)
-admit()
-*)
+let allocs_subset (g:heap{Seq.length (objects2 0UL g) > 0}) 
+                  (g':heap{Seq.length (objects2 0UL g') > 0}) =
+ let allocs = (get_allocated_block_addresses g) in
+ let allocs' = (get_allocated_block_addresses g') in
+  (forall x. Seq.mem x allocs' ==>
+             Seq.mem x allocs)
 
+let allocs_wosize_tag_reads_equal (g:heap{Seq.length (objects2 0UL g) > 0}) 
+                                  (g':heap{Seq.length (objects2 0UL g') > 0}) =
+ let allocs = (get_allocated_block_addresses g) in
+ let allocs' = (get_allocated_block_addresses g') in
+  (forall x. Seq.mem x allocs' ==>
+              getWosize(read_word g x) == getWosize(read_word g' x)) /\
+  (forall x. Seq.mem x allocs' ==>
+              getTag(read_word g x) == getTag(read_word g' x))
 
+ let fields_within_limit_allocs (g:heap{Seq.length (objects2 0UL g) > 0}) =
+ (forall x. Seq.mem x (get_allocated_block_addresses g) ==> 
+        is_fields_within_limit1 x (getWosize (read_word g x)))
 
 
 #restart-solver
+
+ let allocs_wosize_tag_reads_equal_lemma (h_index: hp_addr)
+                                         (g:heap{Seq.length (objects2 0UL g) > 0}) 
+                                         (g':heap{Seq.length (objects2 0UL g') > 0})
+                                         
+                        : Lemma
+                          (requires (allocs_wosize_tag_reads_equal g g' /\
+                                    (Seq.mem h_index (get_allocated_block_addresses g')) /\
+                                     allocs_subset g g' /\
+                                     field_reads_equal1 g g'
+                          ))
+                          (ensures True)  =
+ 
+ let allocs = (get_allocated_block_addresses g) in
+ let allocs' = (get_allocated_block_addresses g') in
+ assert (forall x. Seq.mem x allocs' ==>
+                    Seq.mem x allocs);
+ assert (Seq.mem h_index (get_allocated_block_addresses g'));
+ assert (Seq.mem h_index (get_allocated_block_addresses g));
+ assert (allocs_wosize_tag_reads_equal g g');
+ assert (forall x. Seq.mem x allocs' ==>
+              getTag(read_word g x) == getTag(read_word g' x));
+ assert (Seq.mem h_index allocs');
+ assert (getTag(read_word g h_index) == getTag(read_word g' h_index));
+ assert (field_reads_equal1 g g');
+ assert (forall x y. Seq.mem x (get_allocated_block_addresses g') /\ 
+                Usize.v y >= Usize.v x + Usize.v mword /\
+                Usize.v y <= Usize.v x + (Usize.v (getWosize (read_word g x)) * Usize.v mword) ==>
+                                                                     read_word g y == read_word g' y);
+  admit()
+
+#restart-solver
+
+#restart-solver
+
+#restart-solver
+
+let field_reads_equal1_lemma (h_index: hp_addr)
+                             (g:heap{Seq.length (objects2 0UL g) > 0}) 
+                             (g':heap{Seq.length (objects2 0UL g') > 0}) 
+                             (wz1: wosize{(is_fields_within_limit1 h_index wz1 /\
+                                           is_fields_contents_within_limit2 h_index wz1 g')}) 
+                                                     
+                             (wz: wosize{(is_fields_within_limit1 h_index wz /\
+                                          is_fields_contents_within_limit2 h_index wz g)})
+                : Lemma
+                  (requires field_reads_equal1 g g' /\
+                            (wz1 == wz) /\
+                            (Usize.v wz1 > 0) /\
+                            (Usize.v wz1 <= Usize.v (getWosize(read_word g' h_index))) /\
+                             (Usize.v wz <= Usize.v (getWosize(read_word g h_index))) /\
+                             (is_hp_addr (Usize.add h_index (Usize.mul wz1 mword))) /\
+                             (Seq.mem h_index (get_allocated_block_addresses g')) /\
+                             allocs_subset g g'
+                  )
+                  (ensures (read_word g' (Usize.add h_index (Usize.mul wz1 mword)) == 
+                            read_word g (Usize.add h_index (Usize.mul wz1 mword)))) =
+  assert (field_reads_equal1 g g');
+  let s = Usize.add h_index (Usize.mul wz1 mword) in
+  assert (read_word g s == read_word g' s);
+  ()
+
+
+let field_reads_tags_equal_lemma (h_index: hp_addr)
+                             (g:heap{Seq.length (objects2 0UL g) > 0}) 
+                             (g':heap{Seq.length (objects2 0UL g') > 0}) 
+                             (wz1: wosize{(is_fields_within_limit1 h_index wz1 /\
+                                           is_fields_contents_within_limit2 h_index wz1 g')}) 
+                                                     
+                             (wz: wosize{(is_fields_within_limit1 h_index wz /\
+                                          is_fields_contents_within_limit2 h_index wz g)})
+                : Lemma
+                  (requires field_reads_equal1 g g' /\
+                            fields_within_limit_allocs g /\
+                            check_all_block_fields_within_limit2 g (get_allocated_block_addresses g)  /\
+                            (wz1 == wz) /\
+                            (Usize.v wz1 > 0) /\
+                            (Usize.v wz1 <= Usize.v (getWosize(read_word g' h_index))) /\
+                             (Usize.v wz <= Usize.v (getWosize(read_word g h_index))) /\
+                             (is_hp_addr (Usize.add h_index (Usize.mul wz1 mword))) /\
+                             (Seq.mem h_index (get_allocated_block_addresses g')) /\
+                             ( let s = (Usize.add h_index (Usize.mul wz1 mword)) in
+                               (read_word g s == read_word g' s) /\
+                                isPointer s g') /\
+                                allocs_wosize_tag_reads_equal g g' /\
+                                allocs_subset g g' /\
+                                (Seq.mem (hd_address (read_word g' (Usize.add h_index (Usize.mul wz1 mword))))  
+                                     (get_allocated_block_addresses g'))
+                             
+                  )
+                  (ensures (let s = Usize.add h_index (Usize.mul wz1 mword) in
+                            let succ = read_word g' s in
+                            let succ' = read_word g s in
+                            let hdr_succ = hd_address succ in
+                            let hdr_succ1 = hd_address succ' in
+                            let tg = tag_of_object1 hdr_succ g' in
+                            let tg1 = tag_of_object1 hdr_succ1 g in
+                            (tg == tg1)))  =
+ assert (field_reads_equal1 g g');
+ let s = Usize.add h_index (Usize.mul wz1 mword) in
+ assert (read_word g s == read_word g' s);
+ let succ = read_word g' s in
+ let succ' = read_word g s in
+ assert (succ == succ');
+
+ assert (is_hp_addr succ);
+ let hdr_succ = hd_address succ in
+ let hdr_succ1 = hd_address succ' in
+
+ assert (hdr_succ == hdr_succ1);
+
+ let tg = tag_of_object1 hdr_succ g' in
+ let tg1 = tag_of_object1 hdr_succ1 g in
+
+ assert (Seq.mem hdr_succ  (get_allocated_block_addresses g'));
+ assert (tg == tg1);
+ ()
+
+
+(*val is_fields_points_to_blocks2 :   (h_index: hp_addr) ->
+                                     (g:heap{Seq.length (objects2 0UL g) > 0})->
+                                     (wz: wosize{(is_fields_within_limit1 h_index wz /\
+                                               is_fields_contents_within_limit2 h_index wz g)}) ->
+                                     (f':seq Usize.t { (forall x. Seq.mem x f' ==> is_hp_addr x) /\
+                                                    (forall x. Seq.mem x f' ==> 
+                                                     Seq.mem x (get_allocated_block_addresses g))})->
+                                 
+                   Tot (b:bool{b == true <==> is_fields_points_to_blocks2_post_condition h_index g wz f'})
+                   (decreases (Usize.v wz))*)
+
+
+
+#reset-options "--z3rlimit 1000 --max_fuel 0 --max_ifuel 0 --using_facts_from '* -FStar.Seq'"
+
+#push-options "--split_queries always"
+
+#restart-solver
+
+#restart-solver
+
+#restart-solver
+
+#restart-solver 
 
 
 #reset-options "--z3rlimit 500" // --max_fuel 0 --max_ifuel 0 --using_facts_from '* -FStar.Seq'"
@@ -2097,9 +2928,9 @@ let rec check_fields_points_to_blocks2_test (g:heap{Seq.length (objects2 0UL g) 
                                             (f':seq Usize.t { (forall x. Seq.mem x f' ==> Usize.v x >= 0 /\ Usize.v x < heap_size) /\
                                                      (forall x. Seq.mem x f' ==> is_hp_addr x) /\
                                                      (forall x. Seq.mem x f' ==> Seq.mem x (get_allocated_block_addresses g)) /\
-                                                     check_all_block_fields_within_limit2  g f'})
-
-
+                                                     check_all_block_fields_within_limit2  g f'}) 
+                                   
+                              
                                : Tot (b:bool{b == true <==> (forall x. Seq.mem x f' ==>
                                           is_fields_points_to_blocks2 x g (getWosize (read_word g x)) (get_allocated_block_addresses g))})
                                (decreases length' f')  =
@@ -2110,10 +2941,10 @@ let rec check_fields_points_to_blocks2_test (g:heap{Seq.length (objects2 0UL g) 
          let hd = Seq.head f' in
          let tl = Seq.tail f' in
          let wz = getWosize (read_word g hd) in
-
+        
          if Usize.v wz = 0 then
-             check_fields_points_to_blocks2_test g tl
-
+             check_fields_points_to_blocks2_test g tl 
+            
          else
            (
              assert (Usize.v wz > 0);
@@ -2124,12 +2955,12 @@ let rec check_fields_points_to_blocks2_test (g:heap{Seq.length (objects2 0UL g) 
                  assert (Seq.length tl < Seq.length f');
                  length'_lemma f';
                  check_fields_points_to_blocks2_test g tl
-
+                  
              )
              else
                   false
-
-           )
+             
+           )   
 
 
 let rec check_fields_points_to_blocks2 g f' =
@@ -2141,7 +2972,7 @@ let rec check_fields_points_to_blocks2 g f' =
          let tl = Seq.tail f' in
          let wz = getWosize (read_word g hd) in
          assert (Usize.v wz > 0);
-
+         
          assert (is_fields_contents_within_limit2 hd (getWosize (read_word g hd)) g);
              if (is_fields_points_to_blocks2 hd g (getWosize (read_word g hd)) (get_allocated_block_addresses g)) then
              (
@@ -2149,12 +2980,12 @@ let rec check_fields_points_to_blocks2 g f' =
                  assert (Seq.length tl < Seq.length f');
                  length'_lemma f';
                  check_fields_points_to_blocks2 g tl
-
+                  
              )
              else
                   false
-
-
+             
+          
 
 #restart-solver
 
@@ -2192,7 +3023,7 @@ let rec check_fields_points_to_blocks2_lemma  g g' f' f'' =
          let wz1 = getWosize (read_word g' hd) in
          assert (wz == wz1);
          assert (Seq.mem hd f');
-
+       
          assert (Usize.v wz > 0);
             assert (is_fields_contents_within_limit2 hd (getWosize (read_word g hd)) g);
             is_fields_points_to_blocks2_lemma hd g wz (get_allocated_block_addresses g) g' wz1 (get_allocated_block_addresses g');
@@ -2205,7 +3036,7 @@ let rec check_fields_points_to_blocks2_lemma  g g' f' f'' =
               length'_lemma f';
               let _ = check_fields_points_to_blocks2_lemma g g' tl tl' in
               assert(check_fields_points_to_blocks2 g tl == true <==> check_fields_points_to_blocks2 g' tl' == true);
-
+              
               assert (check_fields_points_to_blocks2 g f' == true <==> check_fields_points_to_blocks2 g' f'' == true);
               ()
              )
@@ -2215,13 +3046,13 @@ let rec check_fields_points_to_blocks2_lemma  g g' f' f'' =
                assert (check_fields_points_to_blocks2 g f' == true <==> check_fields_points_to_blocks2 g' f'' == true);
                ()*)
                ()
-
+               
              )
-
+         
 #reset-options "--z3rlimit 500"
 
 let rec check_well_formed_closure_objs g f =
-  if Seq.length f = 0 then
+  if Seq.length f = 0 then 
     true
   else
   (
@@ -2251,7 +3082,7 @@ let rec check_well_formed_closure_objs g f =
                   Usize.v (extract_start_env_bits (closinfo_val_from_closure_object g (f_address obj))) <= Usize.v (wosize_of_object1 obj g) /\
                   Usize.v (extract_start_env_bits (closinfo_val_from_closure_object g (f_address obj))) >= 1);
            assert (f == Seq.cons obj rest_f);
-           (*assert (forall x. Seq.mem x rest_f ==> Usize.v (tag_of_object1 x g) = closure_tag ==>
+           (*assert (forall x. Seq.mem x rest_f ==> Usize.v (tag_of_object1 x g) = closure_tag ==> 
                                        Usize.v (wosize_of_object1 x g) >= 2 /\
                                        is_hp_addr (extract_start_env_bits (closinfo_val_from_closure_object g (f_address x))) /\
                                        Usize.v (extract_start_env_bits (closinfo_val_from_closure_object g (f_address x))) + 1 <= Usize.v (wosize_of_object1 x g) /\
@@ -2267,8 +3098,8 @@ let rec check_well_formed_closure_objs g f =
          )
       )
       else
-      (
-        let b = false in
+      ( 
+        let b = false in 
         assert (b == true <==> closure_obj_props g f);
         b
       )
@@ -2282,7 +3113,7 @@ let rec check_well_formed_closure_objs g f =
     )
   )
 
-let get_succ_address g h_index wz i =
+let get_succ_address g h_index wz i = 
  let succ_address = Usize.add h_index (Usize.mul i mword) in
  assert (is_hp_addr succ_address);
  assert (Usize.v succ_address >= Usize.v mword);
@@ -2307,7 +3138,7 @@ let wosize_succ g h_index wz i =
 wosize_of_object1 (hdr_address_succ_ptr g h_index wz i) g
 
 let tag_succ g h_index wz i =
-tag_of_object1 (hdr_address_succ_ptr g h_index wz i) g
+tag_of_object1 (hdr_address_succ_ptr g h_index wz i) g 
 
 (*predicate that ensures substraction is possible from the current succ pointer (infix) to reach its actual closure parent*)
 
@@ -2330,13 +3161,13 @@ let infix_parent g h_index wz i =
  Usize.sub (get_succ_value g h_index wz i) (Usize.mul (wosize_succ g h_index wz i) mword)
 
 (*header address of the parent of the infix object*)
-let hdr_infix_parent g h_index wz i =
+let hdr_infix_parent g h_index wz i = 
  hd_address (infix_parent g h_index wz i)
-
+ 
 
 let closinfo_val_from_closure_object_lemma g f_addr g' =
  let hdr_f_addr = hd_address f_addr in
- let offst1 = mword in
+ let offst1 = Usize.mul 1UL mword in
  let wz = wosize_of_object1 hdr_f_addr g in
  assert (is_fields_within_limit1 hdr_f_addr wz);
  let s1 = Usize.add f_addr offst1 in
@@ -2349,7 +3180,7 @@ let closinfo_val_from_closure_object_lemma g f_addr g' =
  ()
 
 let rec check_well_formed_closure_objs_lemma g g' f f'' =
-  if Seq.length f = 0 then
+  if Seq.length f = 0 then 
     ()
   else
   (
@@ -2361,9 +3192,9 @@ let rec check_well_formed_closure_objs_lemma g g' f f'' =
 
     assert (obj == obj1);
     assert (rest_f == rest_f1);
-
+    
     assert (Seq.length rest_f < Seq.length f);
-
+    
     let tg = tag_of_object1 obj g in
     let wz = wosize_of_object1 obj g in
 
@@ -2372,7 +3203,7 @@ let rec check_well_formed_closure_objs_lemma g g' f f'' =
 
     assert (wz == wz1);
     assert (tg == tg1);
-
+    
     if (Usize.v tg = closure_tag) then
     (
       if (Usize.v wz >= 2) then
@@ -2384,7 +3215,7 @@ let rec check_well_formed_closure_objs_lemma g g' f f'' =
                          is_fields_within_limit1 (hd_address f_addr) (wosize_of_object1 (hd_address f_addr) g));
          let clos_info = closinfo_val_from_closure_object g f_addr in
          let start_env = extract_start_env_bits clos_info in
-
+         
          let clos_info1 = closinfo_val_from_closure_object g' f_addr in
          let start_env1 = extract_start_env_bits clos_info1 in
 
@@ -2394,28 +3225,28 @@ let rec check_well_formed_closure_objs_lemma g g' f f'' =
          if is_hp_addr start_env && Usize.v start_env <= Usize.v wz && Usize.v start_env >= 1 then
          (
            let b = check_well_formed_closure_objs g rest_f in
-
+          
            check_well_formed_closure_objs_lemma g g' rest_f rest_f1;
            ()
          )
          else
          (
            let b = false in
-
+           
            ()
          )
       )
       else
-      (
-        let b = false in
-
+      ( 
+        let b = false in 
+        
         ()
       )
     )
     else
     (
       let b = check_well_formed_closure_objs g rest_f in
-
+      
       check_well_formed_closure_objs_lemma g g' rest_f rest_f1;
       ()
     )
@@ -2439,53 +3270,553 @@ let check_well_formed_closure_objs_lemma2_prop  (g:heap{Seq.length (objects2 0UL
                                                  (f:seq Usize.t {(forall x. Seq.mem x f ==> Usize.v x >= 0 /\ Usize.v x < heap_size) /\
                                                                   (forall x. Seq.mem x f ==> Usize.v x % Usize.v mword == 0) /\
                                                                   (forall x. Seq.mem x f ==> Seq.mem x (get_allocated_block_addresses g)) /\
-
+                                                                   
                                                                   (forall x. Seq.mem x f ==> is_fields_within_limit1 x (getWosize (read_word g x)))})=
-  forall x. (Seq.mem x f /\ (Usize.v (tag_of_object1 x g) = closure_tag)) ==>
+  forall x. (Seq.mem x f /\ (Usize.v (tag_of_object1 x g) = closure_tag)) ==> 
                       (Usize.v (wosize_of_object1 x g) >= 2 /\
                       is_hp_addr (extract_start_env_bits (closinfo_val_from_closure_object g (f_address x))) /\
                       Usize.v (extract_start_env_bits (closinfo_val_from_closure_object g (f_address x))) + 1 <= Usize.v (wosize_of_object1 x g) /\
-                      Usize.v (extract_start_env_bits (closinfo_val_from_closure_object g (f_address x))) >= 1)
+                      Usize.v (extract_start_env_bits (closinfo_val_from_closure_object g (f_address x))) >= 1)                                    
 
 
 #reset-options "--z3rlimit 500"
 
 #restart-solver
 
+#reset-options "--z3rlimit 500"
+
+#restart-solver
+
+#restart-solver
+
+#restart-solver
+
+#restart-solver
+
+#restart-solver
+
+#restart-solver
+
+
+(*let sweep_proving_lemma  (g:heap{Seq.length (objects2 0UL g) > 0 /\
+                                 (forall i x.  Seq.mem x (get_allocated_block_addresses g) /\
+                                                        (Usize.v i > 0 /\ Usize.v i <= Usize.v (getWosize (read_word g x))) ==> 
+                                                    (Usize.v x  + (Usize.v i  * Usize.v mword)) % Usize.v mword == 0)})
+                         (g':heap{Seq.length (objects2 0UL g') > 0 /\
+                                  (forall i x.  Seq.mem x (get_allocated_block_addresses g') /\
+                                                        (Usize.v i > 0 /\ Usize.v i <= Usize.v (getWosize (read_word g' x))) ==> 
+                                                    (Usize.v x  + (Usize.v i  * Usize.v mword)) % Usize.v mword == 0) /\
+                                  (forall x. Seq.mem x (get_allocated_block_addresses g') ==> Seq.mem x (get_allocated_block_addresses g))}) =
+
+ 
+ (forall x. Seq.mem x (get_allocated_block_addresses g') ==>
+       
+          (forall i. (Usize.v i > 0 /\ Usize.v i <= Usize.v (getWosize(read_word g' x))) ==>
+        
+             (isPointer (Usize.add x (Usize.mul i mword)) g' ==> 
+                    is_hp_addr (Usize.add x (Usize.mul i mword))
+                   (*tag_of_object1 (hd_address (read_word g' (Usize.add x (Usize.mul i mword)))) g' == 
+                     tag_of_object1 (hd_address (read_word g (Usize.add x (Usize.mul i mword)))) g /\
+                   wosize_of_object1 (hd_address (read_word g' (Usize.add x (Usize.mul i mword)))) g' == 
+                     wosize_of_object1 (hd_address (read_word g (Usize.add x (Usize.mul i mword)))) g*))))*)
+
+#restart-solver
+
+#restart-solver
+
+#restart-solver
+
+#restart-solver
+
+#restart-solver
+
+(*This post-condition should be proved from sweep*)
+let field_reads_hd_equal1 (g:heap{Seq.length (objects2 0UL g) > 0}) 
+                          (g':heap{Seq.length (objects2 0UL g') > 0}) =
+  
+  (forall x y. Seq.mem x (get_allocated_block_addresses g') /\ 
+                Usize.v y >= Usize.v x + Usize.v mword /\
+                Usize.v y <= Usize.v x + (Usize.v (getWosize (read_word g x)) * Usize.v mword) ==>
+                 is_hp_addr (read_word g' y) /\ (isPointer y g') ==> 
+                 is_hp_addr (read_word g y) /\
+                 Usize.v (read_word g y) >= Usize.v mword /\
+                 Usize.v (read_word g' y) >= Usize.v mword /\
+                 is_hp_addr (hd_address (read_word g y)) /\
+                 is_hp_addr (hd_address (read_word g' y))) /\
+  
+  (forall x y. Seq.mem x (get_allocated_block_addresses g') /\ 
+                Usize.v y >= Usize.v x + Usize.v mword /\
+                Usize.v y <= Usize.v x + (Usize.v (getWosize (read_word g x)) * Usize.v mword) ==>
+                is_hp_addr (read_word g' y) /\ (isPointer y g') ==> 
+                                                                    tag_of_object1 (hd_address (read_word g y)) g ==  tag_of_object1 (hd_address (read_word g' y)) g' /\
+                                                                    wosize_of_object1 (hd_address (read_word g y)) g == wosize_of_object1 (hd_address (read_word g' y)) g')
+
+#restart-solver
+
+#restart-solver
+
+#restart-solver
+
+#restart-solver
+
+#restart-solver
+
+let field_mem_props (g:heap{Seq.length (objects2 0UL g) > 0}) 
+                    (g':heap{Seq.length (objects2 0UL g') > 0 /\
+                             field_reads_hd_equal1 g g'}) =
+  
+  (forall x y. Seq.mem x (get_allocated_block_addresses g') /\ 
+                Usize.v y >= Usize.v x + Usize.v mword /\
+                Usize.v y <= Usize.v x + (Usize.v (getWosize (read_word g x)) * Usize.v mword) /\
+                is_hp_addr (read_word g' y) /\ (isPointer y g') ==>
+                
+                 (Usize.v (tag_of_object1 (hd_address (read_word g' y)) g') <> infix_tag ==>
+                    (Seq.mem (hd_address (read_word g' y)) (get_allocated_block_addresses g')))) /\
+
+  (forall x y. Seq.mem x (get_allocated_block_addresses g') /\ 
+                Usize.v y >= Usize.v x + Usize.v mword /\
+                Usize.v y <= Usize.v x + (Usize.v (getWosize (read_word g x)) * Usize.v mword) /\
+                is_hp_addr (read_word g' y) /\ (isPointer y g') ==>  
+                (Usize.v (tag_of_object1 (hd_address (read_word g' y)) g') == infix_tag ==> 
+                 UInt.fits (Usize.v (read_word g' y) - 
+                                                   (Usize.v (wosize_of_object1 (hd_address (read_word g' y)) g') * Usize.v mword)) Usize.n /\
+                 (let actual_succ = (Usize.sub (read_word g' y) 
+                                        (Usize.mul (wosize_of_object1 (hd_address (read_word g' y)) g') mword)) in
+                   Usize.v actual_succ >= Usize.v mword /\
+                   (is_hp_addr actual_succ) /\
+                   (Usize.v (tag_of_object1 (hd_address actual_succ) g') == closure_tag) /\
+                   Seq.mem (hd_address actual_succ) (get_allocated_block_addresses g'))))
+          
+#restart-solver
+
+#restart-solver
+
+#restart-solver
+
+#restart-solver
+
+(*let rec is_fields_points_to_blocks2_lemma_for_sweep  (h_index: hp_addr) 
+                                                     (g:heap{Seq.length (objects2 0UL g) > 0}) 
+                                                     (g':heap{Seq.length (objects2 0UL g') > 0}) 
+                                                     (wz1: wosize{(is_fields_within_limit1 h_index wz1 /\
+                                                                   is_fields_contents_within_limit2 h_index wz1 g')}) 
+                                                     
+                                                     (wz: wosize{(is_fields_within_limit1 h_index wz /\
+                                                                    is_fields_contents_within_limit2 h_index wz g)})
+                               : Lemma
+                                  (requires 
+                                            (*(wz1 == getWosize (read_word g' h_index)) /\*)
+                                             allocs_subset g g' /\
+                                             
+                                             
+                                             (wz == wz1) /\
+                                             (Usize.v wz1 >= 0) /\
+                                             (Usize.v wz1 <= Usize.v (getWosize(read_word g' h_index))) /\
+                                             (Usize.v wz <= Usize.v (getWosize(read_word g h_index))) /\
+                                             allocs_wosize_tag_reads_equal g g' /\
+                                             fields_within_limit_allocs g /\
+                                             check_all_block_fields_within_limit2 g (get_allocated_block_addresses g) /\
+                                             check_fields_points_to_blocks2 g (get_allocated_block_addresses g) /\
+                                             check_well_formed_closure_objs g (get_allocated_block_addresses g) /\
+ 
+                                            (Seq.mem h_index (get_allocated_block_addresses g')) /\
+
+                                            field_reads_equal1 g g' /\
+                                            field_reads_hd_equal1 g g' /\
+
+                                            is_fields_points_to_blocks2 h_index g wz
+                                                                        (get_allocated_block_addresses g) /\
+                                            field_mem_props g g'
+                                          )
+                                  (ensures is_fields_points_to_blocks2 h_index g' wz1 
+                                                       (get_allocated_block_addresses g') == true
+                                            )
+                                  (decreases (Usize.v wz1)) = 
+assert (is_hp_addr h_index);
+ if (Usize.v wz1 = 0) then ()
+  else
+  (
+    assert (Usize.v wz1 > 0);
+    //get the successor_index = h_index + wz * mword
+    let s = Usize.add h_index (Usize.mul wz1 mword) in
+    // For recursing, find wz' = wz - 1
+    let wz' = Usize.sub wz1 1UL in
+    let wz'' = Usize.sub wz 1UL in
+    wosize_times_mword_multiple_of_mword wz1;
+    assert (Usize.v (Usize.mul wz1 mword) % Usize.v mword == 0);
+    //assert ((Usize.v h_index + (Usize.v wz1 * Usize.v mword)) % Usize.v mword == 0);
+    
+    sum_of_multiple_of_mword_is_multiple_of_mword h_index (Usize.mul wz1 mword);
+    assert ((Usize.v h_index + (Usize.v wz1 * Usize.v mword)) % Usize.v mword == 0);
+    assert (Usize.v s % Usize.v mword == 0);
+    assert (Usize.v s < heap_size);
+    assert (is_hp_addr s);
+    if (isPointer s g') then
+    (
+      
+      lemma_len_slice g' (Usize.v s) ((Usize.v s) + (Usize.v mword));
+      lemma_len_slice g (Usize.v s) ((Usize.v s) + (Usize.v mword));
+      let succ = read_word g' s in
+      let succ' = read_word g s in
+      
+      field_reads_equal1_lemma h_index g g' wz1 wz;
+      assert (succ == succ');
+
+      assert (Usize.v succ >= Usize.v mword);
+      assert (Usize.v succ < heap_size);
+      assert (Usize.v succ % Usize.v mword == 0);
+      assert (is_hp_addr succ);
+    
+      let hdr_succ = hd_address succ in
+      let hdr_succ1 = hd_address succ' in
+      assert (hdr_succ == hdr_succ1);
+      let tg = tag_of_object1 hdr_succ g' in
+      let tg1 = tag_of_object1 hdr_succ1 g in
+
+      let wz_hdr_succ = wosize_of_object1 hdr_succ g' in
+      let wz_hdr_succ1 = wosize_of_object1 hdr_succ1 g in
+
+      assert (allocs_wosize_tag_reads_equal g g');
+      
+      assert ((hd_address (read_word g' (Usize.add h_index (Usize.mul wz1 mword)))) ==
+              (hd_address (read_word g (Usize.add h_index (Usize.mul wz mword))))); 
+
+      assert (isPointer (Usize.add h_index (Usize.mul wz1 mword)) g' ==> 
+                   tag_of_object1 (hd_address (read_word g' (Usize.add h_index (Usize.mul wz1 mword)))) g' == tag_of_object1 (hd_address (read_word g (Usize.add h_index (Usize.mul wz1 mword)))) g /\
+                   wosize_of_object1 (hd_address (read_word g' (Usize.add h_index (Usize.mul wz1 mword)))) g' == wosize_of_object1 (hd_address (read_word g (Usize.add h_index (Usize.mul wz1 mword)))) g);
+
+
+      assert (isPointer (Usize.add h_index (Usize.mul wz1 mword)) g' ==> 
+                   tag_of_object1 (hd_address (read_word g' s)) g' == tag_of_object1 (hd_address (read_word g s)) g /\
+                   wosize_of_object1 (hd_address (read_word g' s)) g' == wosize_of_object1 (hd_address (read_word g s)) g);
+
+
+      assert (isPointer (Usize.add h_index (Usize.mul wz1 mword)) g' ==> 
+                   tag_of_object1 (hd_address succ) g' == tag_of_object1 (hd_address succ) g /\
+                   wosize_of_object1 (hd_address succ) g' == wosize_of_object1 (hd_address succ) g);
+
+
+      assert (isPointer (Usize.add h_index (Usize.mul wz1 mword)) g' ==> 
+                   tag_of_object1 (hd_address succ) g' == tag_of_object1 (hd_address succ) g /\
+                   wosize_of_object1 (hd_address succ) g' == wosize_of_object1 (hd_address succ) g);
+
+
+      assert (isPointer (Usize.add h_index (Usize.mul wz1 mword)) g' ==> 
+                   tag_of_object1 hdr_succ g' == tag_of_object1 hdr_succ1 g /\
+                   wosize_of_object1 hdr_succ g' == wosize_of_object1 hdr_succ1 g);
+
+
+      assert (isPointer (Usize.add h_index (Usize.mul wz1 mword)) g' ==> 
+                   tg == tg1 /\
+                   wz_hdr_succ == wz_hdr_succ1);
+
+
+      assert (isPointer s g' ==> 
+                   tg == tg1 /\
+                   wz_hdr_succ == wz_hdr_succ1);
+      
+      if (Usize.v tg <> infix_tag) then
+      (
+        assert (Seq.mem hdr_succ (get_allocated_block_addresses g));
+        
+        assert (tg == tg1);
+        
+        assert (Seq.mem h_index (get_allocated_block_addresses g'));
+        assert (Usize.v s >= Usize.v h_index + Usize.v mword /\
+                Usize.v s <= Usize.v h_index + (Usize.v (getWosize (read_word g' h_index)) * Usize.v mword));
+        
+        assert (is_hp_addr (read_word g' s) /\ (isPointer s g'));
+
+        assert (Usize.v (tag_of_object1 (hd_address (read_word g' s)) g') <> infix_tag); 
+
+        assert (Seq.mem (hd_address (read_word g' s)) (get_allocated_block_addresses g'));
+
+        assert (Seq.mem hdr_succ (get_allocated_block_addresses g'));
+        
+        is_fields_points_to_blocks2_lemma_for_sweep h_index g g' wz' wz'';
+        assert (is_fields_points_to_blocks2 h_index g' wz' 
+                                                       (get_allocated_block_addresses g'));
+        assert (is_fields_points_to_blocks2 h_index g' wz1 
+                                                       (get_allocated_block_addresses g'));
+        ()
+      )
+      else
+      (
+        assert (Usize.v tg == infix_tag);
+      
+        assert (wz_hdr_succ == wz_hdr_succ1);
+
+        let wz_succ_offset = Usize.mul wz_hdr_succ mword in
+        
+        assert (is_fields_points_to_blocks2_post_condition h_index g wz (get_allocated_block_addresses g)); 
+
+        assert (
+                  (Usize.v (tag_of_object1 (hd_address (read_word g (Usize.add h_index (Usize.mul wz1 mword)))) g) == infix_tag) /\
+                  (UInt.fits (Usize.v (read_word g (Usize.add h_index (Usize.mul wz1 mword))) - 
+                                                   (Usize.v (wosize_of_object1 (hd_address (read_word g (Usize.add h_index (Usize.mul wz1 mword)))) g) * Usize.v mword)) Usize.n) /\
+                    (
+                                                       (let actual_succ = (Usize.sub (read_word g (Usize.add h_index (Usize.mul wz1 mword))) 
+                                                       (Usize.mul (wosize_of_object1 (hd_address (read_word g (Usize.add h_index (Usize.mul wz1 mword)))) g) mword)) in
+                                                        (Usize.v actual_succ >= Usize.v mword) /\
+                                                        (is_hp_addr actual_succ) /\
+                                                        (Usize.v (tag_of_object1 (hd_address actual_succ) g) == closure_tag) /\
+                                                        (Seq.mem (hd_address actual_succ) (get_allocated_block_addresses g)))
+                   ));
+
+        
+        assert (UInt.fits (Usize.v (read_word g (Usize.add h_index (Usize.mul wz1 mword))) - 
+                                                   (Usize.v (wosize_of_object1 (hd_address (read_word g (Usize.add h_index (Usize.mul wz1 mword)))) g) * Usize.v mword)) Usize.n);
+        assert (UInt.fits (Usize.v (read_word g s) - 
+                                                   (Usize.v (wosize_of_object1 (hd_address (read_word g (Usize.add h_index (Usize.mul wz1 mword)))) g) * Usize.v mword)) Usize.n);
+
+        assert (UInt.fits (Usize.v (read_word g s) - 
+                                                   (Usize.v (wosize_of_object1 (hd_address (read_word g s)) g) * Usize.v mword)) Usize.n);
+        
+        assert (UInt.fits (Usize.v succ' - (Usize.v (wosize_of_object1 (hd_address succ') g) * Usize.v mword)) Usize.n);
+                                                   
+        assert (UInt.fits (Usize.v succ' - (Usize.v wz_hdr_succ1 * Usize.v mword)) Usize.n);
+
+        assert (UInt.fits (Usize.v succ - (Usize.v wz_hdr_succ * Usize.v mword)) Usize.n);
+
+        
+
+        let actual_succ' = Usize.sub succ' (Usize.mul wz_hdr_succ1 mword) in
+
+        let actual_succ = Usize.sub succ (Usize.mul wz_hdr_succ mword) in
+        
+        
+
+        assert (actual_succ' == actual_succ);
+        
+        assert  ((Usize.v actual_succ >= Usize.v mword) /\
+                 (is_hp_addr actual_succ));
+        assert (Usize.v (tag_of_object1 (hd_address actual_succ') g) == closure_tag);
+
+        assert (Usize.v (tag_of_object1 (hd_address actual_succ) g') == Usize.v (tag_of_object1 (hd_address actual_succ) g));
+
+        assert (Usize.v (tag_of_object1 (hd_address actual_succ) g') == closure_tag);
+
+        assert (Seq.mem (hd_address actual_succ) (get_allocated_block_addresses g));
+
+        assert (Seq.mem (hd_address actual_succ) (get_allocated_block_addresses g'));
+        
+        is_fields_points_to_blocks2_lemma_for_sweep h_index g g' wz' wz'';
+        assert (is_fields_points_to_blocks2 h_index g' wz' 
+                                                       (get_allocated_block_addresses g'));
+        assert (is_fields_points_to_blocks2 h_index g' wz1 
+                                                       (get_allocated_block_addresses g'));
+
+        ()                                              
+      )
+    )
+    else
+    (
+      assert (~(isPointer s g'));
+      
+      assert ((is_fields_within_limit1 h_index wz' /\
+               is_fields_contents_within_limit2 h_index wz' g'));
+      is_fields_points_to_blocks2_lemma_for_sweep  h_index g g' wz' wz'';
+      assert (is_fields_points_to_blocks2 h_index g' wz' 
+                                                       (get_allocated_block_addresses g'));
+      assert (is_fields_points_to_blocks2 h_index g' wz1 
+                                                       (get_allocated_block_addresses g'));
+      ()
+    )
+ 
+  )
+
+  for allocated objects in g1, their field pointers cannot point to the fp block.
+  all allocs in g2 ===> allocs in g1
+  all allocs in g2 ==> field values in g1 == field values in g2
+
+  
+  
+  for allocated objects in g2, their field pointers cannot point to the fp block.
+
+  to prove
+
+  for all allocs in g2 ===> field pointers points to allocs in g2
+
+
+  color changes, first field of certain objects changes, in coalescing, object size also change.
+
+
+  The changes still preserves the property that we want to prove.
+
+  color chane and wosize change ===> does not affect first field
+
+  free list manipulation ====> we need to prove that it does not affect well formedness.
+
+  any allocated object never points to an fp ----> invariant since fp is manipulated by the sweep. Initailly fp is null and allocs 
+     never points to null. So true initially.
+
+  When we encounter a blue or white object, fp will point to that object. But after mark, black obj never points to blue or white. 
+  therefore allocated objs never point to fp object after mark.
+
+  From sweep function, we need to prove this in place. Bring this property outside as a post condition of sweep through a lemma.
+
+
+  After every iteration of sweep body, the allocated objects in the current state of the heap (during) never points to fp.
+
+    g1 ---> 2 invariants --- co-inductive proof, one property by itself is not inductive. But together they preserve.
+    1. black objects in g1 points to 
+    2. After every iteration of sweep body, the black objects in g1 never points to fp. 
+
+
+    Overall after sweep,
+
+    allocs of g2 <==> white in g2
+    blacks in g1 <==> whites in g2
+    field pointers of black <==> whites in g2
+ ---------------------
+    blacks objects in g1 points to allocated objects in the current state of the heap ---> this to be proved (line 2874 is needed)
+
+    black objects in g1 points to allocated objects in g2
+
+    blacks in g1 <==> whites in g2
+
+
+
+    the white objects in g2 never points to fp.
+
+    ---------------------
+
+    input to sweep body
+    sweep-body
+    g1'
+    allocated object in g1' points to allocated objects in g1'
+    
+
+     -----> sweep-body g1' ----> rest of sweep g2'  ----> g2
+
+---------------------------------------------------------------------------
+
+
+
+
+*)
+#restart-solver
+
+#restart-solver
+
+let field_mem_props_pre (g:heap{Seq.length (objects2 0UL g) > 0}) 
+                          (g':heap{Seq.length (objects2 0UL g') > 0}) =
+  
+  (forall x y. Seq.mem x (get_allocated_block_addresses g') /\ 
+                Usize.v y >= Usize.v x + Usize.v mword /\
+                Usize.v y <= Usize.v x + (Usize.v (getWosize (read_word g x)) * Usize.v mword) ==>
+                 is_hp_addr (read_word g' y) /\ (isPointer y g') ==> 
+                 is_hp_addr (read_word g y) /\
+                 Usize.v (read_word g y) >= Usize.v mword /\
+                 Usize.v (read_word g' y) >= Usize.v mword /\
+                 is_hp_addr (hd_address (read_word g y)) /\
+                 is_hp_addr (hd_address (read_word g' y)))
+
+let field_mem_props1 (g:heap{Seq.length (objects2 0UL g) > 0}) 
+                    (g':heap{Seq.length (objects2 0UL g') > 0 /\ field_mem_props_pre g g'}) =
+  
+  (forall x y. Seq.mem x (get_allocated_block_addresses g') /\ 
+                Usize.v y >= Usize.v x + Usize.v mword /\
+                Usize.v y <= Usize.v x + (Usize.v (getWosize (read_word g x)) * Usize.v mword) /\
+                is_hp_addr (read_word g' y) /\ (isPointer y g') ==>
+                
+                 (Usize.v (tag_of_object1 (hd_address (read_word g' y)) g') <> infix_tag ==>
+                    (Seq.mem (hd_address (read_word g' y)) (get_allocated_block_addresses g')))) /\
+
+  (forall x y. Seq.mem x (get_allocated_block_addresses g') /\ 
+                Usize.v y >= Usize.v x + Usize.v mword /\
+                Usize.v y <= Usize.v x + (Usize.v (getWosize (read_word g x)) * Usize.v mword) /\
+                is_hp_addr (read_word g' y) /\ (isPointer y g') ==>  
+                (Usize.v (tag_of_object1 (hd_address (read_word g' y)) g') == infix_tag ==> 
+                 UInt.fits (Usize.v (read_word g' y) - 
+                                                   (Usize.v (wosize_of_object1 (hd_address (read_word g' y)) g') * Usize.v mword)) Usize.n /\
+                 (let actual_succ = (Usize.sub (read_word g' y) 
+                                        (Usize.mul (wosize_of_object1 (hd_address (read_word g' y)) g') mword)) in
+                   Usize.v actual_succ >= Usize.v mword /\
+                   (is_hp_addr actual_succ) /\
+                   (Usize.v (tag_of_object1 (hd_address actual_succ) g') == closure_tag) /\
+                   Seq.mem (hd_address actual_succ) (get_allocated_block_addresses g'))))
+
+
+let is_fields_points_to_blocks2_lemma_for_sweep1  (h_index: hp_addr) 
+                                                     (g:heap{Seq.length (objects2 0UL g) > 0}) 
+                                                     (g':heap{Seq.length (objects2 0UL g') > 0}) 
+                                                     (wz1: wosize{(is_fields_within_limit1 h_index wz1 /\
+                                                                   is_fields_contents_within_limit2 h_index wz1 g')}) 
+                                                     
+                                                     (wz: wosize{(is_fields_within_limit1 h_index wz /\
+                                                                    is_fields_contents_within_limit2 h_index wz g)})
+                               : Lemma
+                                  (requires 
+                                            (*(wz1 == getWosize (read_word g' h_index)) /\*)
+                                             allocs_subset g g' /\
+                                             
+                                             
+                                             (wz == wz1) /\
+                                             (Usize.v wz1 >= 0) /\
+                                             (Usize.v wz1 <= Usize.v (getWosize(read_word g' h_index))) /\
+                                             (Usize.v wz <= Usize.v (getWosize(read_word g h_index))) /\
+                                             allocs_wosize_tag_reads_equal g g' /\
+                                             fields_within_limit_allocs g /\
+                                             check_all_block_fields_within_limit2 g (get_allocated_block_addresses g) /\
+                                             check_fields_points_to_blocks2 g (get_allocated_block_addresses g) /\
+                                             check_well_formed_closure_objs g (get_allocated_block_addresses g) /\
+ 
+                                            (Seq.mem h_index (get_allocated_block_addresses g')) /\
+
+                                            field_reads_equal1 g g' /\
+                                            field_reads_hd_equal1 g g' /\
+
+                                            is_fields_points_to_blocks2 h_index g wz
+                                                                        (get_allocated_block_addresses g) /\
+                                            field_mem_props1 g g'
+                                          )
+                                  (ensures is_fields_points_to_blocks2 h_index g' wz1 
+                                                       (get_allocated_block_addresses g') == true
+                                            ) = ()
 
 let well_formed_heap2 g =
    let f = objects2 0UL g in
-
+   
   if length f > 0 then
   (
      let f' = get_allocated_block_addresses g in
-     if check_all_block_fields_within_limit2 g f' &&
-        check_fields_points_to_blocks2 g f' &&
+     if check_all_block_fields_within_limit2 g f' && 
+        check_fields_points_to_blocks2 g f' && 
          check_well_formed_closure_objs g f' then
        true
      else
-      false
+      false 
   )
-
+ 
   else
-   false
-
-
-#restart-solver
-
-#reset-options "--z3rlimit 50 --max_fuel 0 --max_ifuel 0 --using_facts_from '* -FStar.Seq'"
-
-#restart-solver
+   false 
 
 #reset-options "--z3rlimit 500"
 
 #restart-solver
 
-#restart-solver
+
+
+
+
+
+
+#restart-solver 
+
+#reset-options "--z3rlimit 50 --max_fuel 0 --max_ifuel 0 --using_facts_from '* -FStar.Seq'"
+
+#restart-solver 
+
+#reset-options "--z3rlimit 500"
 
 #restart-solver
 
-let objects2_cons_lemma1 h_index g h_index_new =
+#restart-solver 
+
+#restart-solver
+
+let objects2_cons_lemma1 h_index g h_index_new = 
  let wz =  getWosize (read_word g h_index) in
  let h_index_new =  Usize.add h_index (Usize.mul (Usize.add wz 1UL) mword) in
 
@@ -2498,7 +3829,7 @@ let objects2_cons_lemma1 h_index g h_index_new =
     (
        assert (Usize.v h_index_new == heap_size);
        let f = Seq.create 1 h_index in
-
+       
        G.is_vertex_set_lemma2 f;
        assert (Seq.length f > 0 /\ (Usize.v h_index_new < heap_size) ==> Seq.mem h_index_new f);
        assert (forall x. Seq.mem x (objects2 h_index g) <==> x == h_index \/ (Seq.mem x (objects2 h_index_new g)));
@@ -2513,12 +3844,12 @@ let objects2_cons_lemma1 h_index g h_index_new =
       assert (is_hp_addr h_index_new);
       let f' =  objects2 h_index_new g in
       objects2_mem_lemma1 h_index_new g;
-      if length f' = 0 then
+      if length f' = 0 then 
       (
         assert (Seq.length f' > 0 /\ (Usize.v h_index_new < heap_size) ==> Seq.mem h_index_new f');
-
+       
         ()
-
+        
       )
        else
        (
@@ -2527,8 +3858,8 @@ let objects2_cons_lemma1 h_index g h_index_new =
          assert (Seq.length f'' > 0 /\ (Usize.v h_index_new < heap_size) ==> Seq.mem h_index_new f'');
          G.is_vertex_set_cons h_index f';
          assert (Seq.length f'' > 0 /\ (Usize.v h_index_new < heap_size) ==> Seq.mem h_index_new f'');
-         assert (Seq.length (objects2 h_index g) > 0 /\
-                        Usize.v h_index_new < heap_size ==>
+         assert (Seq.length (objects2 h_index g) > 0 /\ 
+                        Usize.v h_index_new < heap_size ==> 
                          (objects2 h_index g) == Seq.cons h_index (objects2 h_index_new g));
          //assert (forall x. Seq.mem x (objects2 h_index g) <==> x == h_index \/ (Seq.mem x (objects2 h_index_new g)));
          ()
@@ -2551,14 +3882,14 @@ let rec objects2_equal_lemma5 g g' h_index =
   let wz1 =  getWosize (read_word g' h_index) in
   assert (wz == wz1);
   assert (Usize.v wz > 0);
-  let h_index_new =  Usize.add h_index (Usize.mul (Usize.add wz 1UL) mword) in
+  let h_index_new =  Usize.add h_index (Usize.mul (Usize.add wz 1UL) mword) in 
   if Usize.v h_index_new <= heap_size then //valid heap condition
   (
     if Usize.v h_index_new = heap_size then // h_index_new == heap_size --> The last block is h_index, So just create a singleton with h_index and return.
     (
        assert (Usize.v h_index_new == heap_size);
        let f = Seq.create 1 h_index in
-
+       
        G.is_vertex_set_lemma2 f;
        ()
     )
@@ -2576,7 +3907,7 @@ let rec objects2_equal_lemma5 g g' h_index =
       objects2_mem_lemma1_app1 h_index g;
       assert (Seq.mem  h_index_new (objects2 0UL g));
       //assert (is_valid_header h_index_new g);
-      let f' =  objects2 h_index_new g in
+      let f' =  objects2 h_index_new g in 
       objects2_equal_lemma5 g g' h_index_new;
       if length f' = 0 then ()
        else
@@ -2604,7 +3935,7 @@ let rec objects2_equal_lemma5 g g' h_index =
 #restart-solver
 
 let objects2_cons_lemma2 h_index g = ()
-
+  
 let objects2_length_lemma3 g h_index h_index_new =
   let wz =  getWosize (read_word g h_index) in
   let h_index_new =  Usize.add h_index (Usize.mul (Usize.add wz 1UL) mword) in
@@ -2618,7 +3949,7 @@ let objects2_length_lemma3 g h_index h_index_new =
     (
        assert (Usize.v h_index_new == heap_size);
        let f = Seq.create 1 h_index in
-
+       
        G.is_vertex_set_lemma2 f;
        assert (Seq.length f > 0 /\ (Usize.v h_index_new < heap_size) ==> Seq.mem h_index_new f);
        assert (forall x. Seq.mem x (objects2 h_index g) <==> x == h_index \/ (Seq.mem x (objects2 h_index_new g)));
@@ -2633,12 +3964,12 @@ let objects2_length_lemma3 g h_index h_index_new =
       assert (is_hp_addr h_index_new);
       let f' =  objects2 h_index_new g in
       objects2_mem_lemma1 h_index_new g;
-      if length f' = 0 then
+      if length f' = 0 then 
       (
         assert (Seq.length f' > 0 /\ (Usize.v h_index_new < heap_size) ==> Seq.mem h_index_new f');
-
+       
         ()
-
+        
       )
        else
        (
@@ -2647,8 +3978,8 @@ let objects2_length_lemma3 g h_index h_index_new =
          assert (Seq.length f'' > 0 /\ (Usize.v h_index_new < heap_size) ==> Seq.mem h_index_new f'');
          G.is_vertex_set_cons h_index f';
          assert (Seq.length f'' > 0 /\ (Usize.v h_index_new < heap_size) ==> Seq.mem h_index_new f'');
-         assert (Seq.length (objects2 h_index g) > 0 /\
-                        Usize.v h_index_new < heap_size ==>
+         assert (Seq.length (objects2 h_index g) > 0 /\ 
+                        Usize.v h_index_new < heap_size ==> 
                          (objects2 h_index g) == Seq.cons h_index (objects2 h_index_new g));
          assert (forall x. Seq.mem x (objects2 h_index g) <==> x == h_index \/ (Seq.mem x (objects2 h_index_new g)));
          assert (Seq.length f' > 0);
@@ -2674,8 +4005,8 @@ let objects2_length_lemma3 g h_index h_index_new =
     assume (Usize.v f_index_new >= heap_size ==> ~(Seq.mem h_index_new (objects2 h_index g)));*)
 let objects2_sweep_lemma1  (h_index: hp_addr)
                            (g:heap{Seq.length (objects2 0UL g) > 0 /\
-                                   Seq.mem h_index (objects2 0UL g)/\
-                                  (Seq.length (objects2 h_index g) > 0)})
+                                   Seq.mem h_index (objects2 0UL g)/\ 
+                                  (Seq.length (objects2 h_index g) > 0)}) 
                   :Lemma
                    (ensures (let wz =  getWosize (read_word g h_index) in
                              let h_index_new =  Usize.add h_index (Usize.mul (Usize.add wz 1UL) mword) in
@@ -2685,19 +4016,19 @@ let objects2_sweep_lemma1  (h_index: hp_addr)
 #restart-solver
 
 let wosize_plus_one_times_mword_multiple_of_mword5 (wz:wosize)
-                     :Lemma
+                     :Lemma 
                       (ensures (Usize.v (Usize.mul (Usize.add wz 1UL) mword) % Usize.v mword == 0)) = ()
 
 let objects2_sweep_lemma2  (h_index: hp_addr)
                            (g:heap{Seq.length (objects2 0UL g) > 0 /\
-                                   Seq.mem h_index (objects2 0UL g)/\
-                                  (Seq.length (objects2 h_index g) > 0)})
+                                   Seq.mem h_index (objects2 0UL g)/\ 
+                                  (Seq.length (objects2 h_index g) > 0)}) 
                   :Lemma
                   (requires (let wz =  getWosize (read_word g h_index) in
                              let h_index_new =  Usize.add h_index (Usize.mul (Usize.add wz 1UL) mword) in
                              let f_index_new =  Usize.add h_index_new mword in
                              Usize.v f_index_new <> heap_size))
-                   (ensures
+                   (ensures 
                    (let wz =  getWosize (read_word g h_index) in
                     let h_index_new =  Usize.add h_index (Usize.mul (Usize.add wz 1UL) mword) in
                     let f_index_new =  Usize.add h_index_new mword in
@@ -2706,7 +4037,7 @@ let wz =  getWosize (read_word g h_index) in
 let h_index_new =  Usize.add h_index (Usize.mul (Usize.add wz 1UL) mword) in
 assert (Seq.mem h_index (objects2 0UL g));
 assert (Seq.length (objects2 0UL g) > 0);
-assert (Seq.length (objects2 0UL g) > 0 ==>
+assert (Seq.length (objects2 0UL g) > 0 ==> 
             (forall x. Seq.mem x (objects2 0UL g) ==> Usize.v (getWosize (read_word g x)) > 0));
 assert  (forall x. Seq.mem x (objects2 0UL g) ==> Usize.v (getWosize (read_word g x)) > 0);
 assert (Usize.v (getWosize (read_word g h_index)) > 0);
@@ -2715,7 +4046,7 @@ assert (Usize.v wz > 0);
 let f_index_new =  Usize.add h_index_new mword in
  wosize_plus_one_times_mword_multiple_of_mword5 wz;
  assert (Usize.v (Usize.mul (Usize.add wz 1UL) mword) % Usize.v mword == 0);
-
+ 
  sum_of_multiple_of_mword_is_multiple_of_mword h_index (Usize.mul (Usize.add wz 1UL) mword);
  sum_of_multiple_of_mword_is_multiple_of_mword h_index_new mword;
 
@@ -2723,7 +4054,7 @@ let f_index_new =  Usize.add h_index_new mword in
  assert (Usize.v f_index_new % Usize.v mword == 0);
  if Usize.v h_index_new <= heap_size then //valid heap condition
   (
-    if Usize.v h_index_new = heap_size then
+    if Usize.v h_index_new = heap_size then 
     (
       assert (Seq.length (objects2 h_index g) == 1);
       assert (Seq.mem h_index (objects2 h_index g));
@@ -2756,10 +4087,10 @@ let f_index_new =  Usize.add h_index_new mword in
 
 let objects2_sweep_lemma3  (h_index: hp_addr)
                            (g:heap{Seq.length (objects2 0UL g) > 0 /\
-                                   Seq.mem h_index (objects2 0UL g)/\
-                                  (Seq.length (objects2 h_index g) > 0)})
+                                   Seq.mem h_index (objects2 0UL g)/\ 
+                                  (Seq.length (objects2 h_index g) > 0)}) 
                   :Lemma
-                   (ensures
+                   (ensures 
                    (let wz =  getWosize (read_word g h_index) in
                     let h_index_new =  Usize.add h_index (Usize.mul (Usize.add wz 1UL) mword) in
                     let f_index_new =  Usize.add h_index_new mword in
@@ -2782,28 +4113,28 @@ objects2_sweep_lemma2 h_index g;
 #restart-solver
 
 (* The below lemma will be used to remove the assume in sweep_with_free_list3
-   assume (~(Seq.mem h_index_new (objects2 h_index g)) /\
-         (Seq.length (objects2 (hd_address f_index) g) > 0) ==>
+   assume (~(Seq.mem h_index_new (objects2 h_index g)) /\ 
+         (Seq.length (objects2 (hd_address f_index) g) > 0) ==> 
            Seq.length (objects2 h_index g) == 1);*)
 
  let objects2_sweep_lemma4  (h_index: hp_addr)
                            (g:heap{Seq.length (objects2 0UL g) > 0 /\
-                                   Seq.mem h_index (objects2 0UL g)/\
-                                  (Seq.length (objects2 h_index g) > 0)})
+                                   Seq.mem h_index (objects2 0UL g)/\ 
+                                  (Seq.length (objects2 h_index g) > 0)}) 
                   :Lemma
-                   (requires
+                   (requires 
                      (let wz =  getWosize (read_word g h_index) in
                      let h_index_new =  Usize.add h_index (Usize.mul (Usize.add wz 1UL) mword) in
                      (~(Seq.mem h_index_new (objects2 h_index g)))))
-
-                   (ensures
+                   
+                   (ensures 
                      (let wz =  getWosize (read_word g h_index) in
                      let h_index_new =  Usize.add h_index (Usize.mul (Usize.add wz 1UL) mword) in
                      let f_index_new =  Usize.add h_index_new mword in
-                     Seq.length (objects2 h_index g) == 1)) =
+                     Seq.length (objects2 h_index g) == 1)) =          
 let wz =  getWosize (read_word g h_index) in
 let h_index_new =  Usize.add h_index (Usize.mul (Usize.add wz 1UL) mword) in
-if Usize.v wz = 0 then
+if Usize.v wz = 0 then 
 (
   ()
 )
@@ -2811,13 +4142,13 @@ else
 (
   if Usize.v h_index_new <= heap_size then
   (
-    if Usize.v h_index_new = heap_size then
+    if Usize.v h_index_new = heap_size then 
     (
       ()
     )
     else
     (
-      assert (Usize.v h_index_new < heap_size);
+      assert (Usize.v h_index_new < heap_size); 
       let f_index_new =  Usize.add h_index_new mword in
       assert (Usize.v h_index_new < heap_size);
       wosize_plus_times_mword_multiple_of_mword3 wz;
@@ -2827,17 +4158,17 @@ else
       assert (h_index_new ==  Usize.add h_index (Usize.mul (Usize.add wz 1UL) mword));
       assert (Usize.v h_index_new == Usize.v h_index + Usize.v (Usize.mul (Usize.add wz 1UL) mword));
       assert (Usize.v h_index_new % Usize.v mword == 0);
-
+      
       assert ((~(Seq.mem h_index_new (objects2 h_index g))));
       assert (is_hp_addr h_index_new);
-      let f' =  objects2 h_index_new g in
+      let f' =  objects2 h_index_new g in 
       lemma_tl h_index f';
       let f'' = cons h_index f' in
       assert (f'' == objects2 h_index g);
       assert ((~(Seq.mem h_index_new (objects2 h_index g))));
       assert (forall x. Seq.mem x (objects2 h_index g) ==> Usize.v x >= Usize.v h_index);
-      assert  ((forall x y. Seq.mem x (objects2 h_index g) /\
-                                                   (Usize.v y >= Usize.v x + Usize.v mword) /\
+      assert  ((forall x y. Seq.mem x (objects2 h_index g) /\ 
+                                                   (Usize.v y >= Usize.v x + Usize.v mword) /\ 
                                                    (Usize.v y <= Usize.v x + (((Usize.v (getWosize (read_word g x)) + 1) * Usize.v mword) - 1)) ==>
                                                    ~(Seq.mem y (objects2 h_index g))));
       assert (Seq.length f' == 0);
@@ -2853,7 +4184,81 @@ else
 )
 
 
+(*
+   assume (Usize.v tg <> infix_tag ==>
+                 Seq.mem (hd_address (read_word g (Usize.add h_index (Usize.mul wz mword))))  
+                                     (get_allocated_block_addresses g'));
 
 
+      assert (Usize.v tg <> infix_tag ==>
+                 Seq.mem (hd_address (read_word g' (Usize.add h_index (Usize.mul wz1 mword))))  
+                                     (get_allocated_block_addresses g'));
+      
+       assume (Usize.v tg1 == infix_tag ==>
+                  (UInt.fits (Usize.v succ - Usize.v (Usize.mul (wosize_of_object1 hdr_succ g) mword)) Usize.n) /\
+                  (Usize.v (Usize.sub succ (Usize.mul (wosize_of_object1 hdr_succ g) mword)) >= Usize.v mword) /\
+                  (is_hp_addr (Usize.sub succ (Usize.mul (wosize_of_object1 hdr_succ g) mword))) /\
+                  Seq.mem (hd_address (Usize.sub succ (Usize.mul (wosize_of_object1 hdr_succ g) mword))) 
+                             (get_allocated_block_addresses g') /\
+                  (Usize.v (tag_of_object1 (hd_address (Usize.sub succ (Usize.mul (wosize_of_object1 hdr_succ g) mword))) g) = closure_tag));
+
+      assume (Usize.v tg1 == infix_tag ==>
+               Usize.sub succ (Usize.mul (wosize_of_object1 hdr_succ g) mword) ==
+               Usize.sub succ (Usize.mul (wosize_of_object1 hdr_succ g') mword));
+
+
+
+
+      assume (Usize.v tg == infix_tag ==>
+                  (UInt.fits (Usize.v succ - Usize.v (Usize.mul (wosize_of_object1 hdr_succ g') mword)) Usize.n) /\
+                  (Usize.v (Usize.sub succ (Usize.mul (wosize_of_object1 hdr_succ g') mword)) >= Usize.v mword) /\
+                  (is_hp_addr (Usize.sub succ (Usize.mul (wosize_of_object1 hdr_succ g') mword))) /\
+                  Seq.mem (hd_address (Usize.sub succ (Usize.mul (wosize_of_object1 hdr_succ g') mword))) 
+                             (get_allocated_block_addresses g') /\
+                  (Usize.v (tag_of_object1 (hd_address (Usize.sub succ (Usize.mul (wosize_of_object1 hdr_succ g') mword))) g') = closure_tag));
+      
+      //assert (Seq.mem hdr_succ (get_allocated_block_addresses g'));
+      //field_reads_tags_equal_lemma h_index g g' wz1 wz;
+  assume (objects2 0UL g == objects2 0UL g');
+      assume ((forall x. Seq.mem x (objects2 0UL g') ==> 
+                            getWosize(read_word g x) == getWosize(read_word g' x)) /\
+              (forall x. Seq.mem x (objects2 0UL g') ==> 
+                            getTag(read_word g x) == getTag(read_word g' x)));*)
+      
+      (*assert (Usize.v tg1 <> infix_tag ==>
+                 Seq.mem hdr_succ1 (get_allocated_block_addresses g));
+      assert (Usize.v tg1 <> infix_tag ==>
+                 Seq.mem hdr_succ1 (objects2 0UL g));
+      assert (Usize.v tg1 <> infix_tag ==>
+                 Seq.mem hdr_succ1 (objects2 0UL g'));
+      (*assert (Usize.v tg1 <> infix_tag ==>
+                 tg == tg1);*)
+
+      assert (Usize.v tg1 <> infix_tag ==>
+                wz_hdr_succ  == wz_hdr_succ1);*)
+
+      (*assert (Usize.v tg1 == infix_tag ==>
+                  (UInt.fits (Usize.v succ - Usize.v (Usize.mul (wosize_of_object1 hdr_succ g) mword)) Usize.n) /\
+                  (Usize.v (Usize.sub succ (Usize.mul (wosize_of_object1 hdr_succ g) mword)) >= Usize.v mword) /\
+                  (is_hp_addr (Usize.sub succ (Usize.mul (wosize_of_object1 hdr_succ g) mword))) /\
+                  Seq.mem (hd_address (Usize.sub succ (Usize.mul (wosize_of_object1 hdr_succ g) mword))) 
+                             (get_allocated_block_addresses g) /\
+                  (Usize.v (tag_of_object1 (hd_address (Usize.sub succ (Usize.mul (wosize_of_object1 hdr_succ g) mword))) g) = closure_tag)); 
+
+      assert (Usize.v tg1 == infix_tag ==>
+                  (UInt.fits (Usize.v succ - Usize.v (Usize.mul (wosize_of_object1 hdr_succ g) mword)) Usize.n) /\
+                  (Usize.v (Usize.sub succ (Usize.mul (wosize_of_object1 hdr_succ g) mword)) >= Usize.v mword) /\
+                  (is_hp_addr (Usize.sub succ (Usize.mul (wosize_of_object1 hdr_succ g) mword))) /\
+                  Seq.mem (hd_address (Usize.sub succ (Usize.mul (wosize_of_object1 hdr_succ g) mword))) 
+                             (objects2 0UL g) /\
+                  (Usize.v (tag_of_object1 (hd_address (Usize.sub succ (Usize.mul (wosize_of_object1 hdr_succ g) mword))) g) = closure_tag)); 
+      
+      assert (Usize.v tg1 == infix_tag ==>
+                  (UInt.fits (Usize.v succ - Usize.v (Usize.mul (wosize_of_object1 hdr_succ g) mword)) Usize.n) /\
+                  (Usize.v (Usize.sub succ (Usize.mul (wosize_of_object1 hdr_succ g) mword)) >= Usize.v mword) /\
+                  (is_hp_addr (Usize.sub succ (Usize.mul (wosize_of_object1 hdr_succ g) mword))) /\
+                  Seq.mem (hd_address (Usize.sub succ (Usize.mul (wosize_of_object1 hdr_succ g) mword))) 
+                             (objects2 0UL g') /\
+                  (Usize.v (tag_of_object1 (hd_address (Usize.sub succ (Usize.mul (wosize_of_object1 hdr_succ g) mword))) g) = closure_tag));*) 
 
 
